thys/HRB-Slicing/Proc/Interpretation.thy
@@ -54,7 +54,7 @@ proof(atomize_elim)
     with `Rep_wf_prog wfp = (prog,procs)` `(Main, n') = r` show ?thesis
       by(fastsimp simp:valid_edge_def)
   next
-    case (ProcCall i px ins outs c l es' rets' l' ins' outs' c' ps es rets)
+    case (ProcCall px ins outs c l es' rets' l' ins' outs' c' ps)
     from ProcCall have "prog,procs \<turnstile> (p,Exit) -(\<lambda>cf. snd cf = (px,Label l'))\<hookleftarrow>\<^bsub>p\<^esub>
       (\<lambda>cf cf'. cf'(rets' [:=] map cf outs'))\<rightarrow> (px,Label l')"
       by(fastsimp intro:ProcReturn)
@@ -149,7 +149,7 @@ proof -
     from this `kind a = Q:r\<hookrightarrow>\<^bsub>p\<^esub>fs` 
     show "\<forall>a'. valid_edge wfp a' \<and> targetnode a' = targetnode a \<longrightarrow>
       (\<exists>Qx rx fsx. kind a' = Qx:rx\<hookrightarrow>\<^bsub>p\<^esub>fsx)"
-    proof(induct n\<equiv>"sourcenode a" et\<equiv>"kind a" n'\<equiv>"targetnode a" rule:PCFG.induct)
+    proof(induct "sourcenode a" "kind a" "targetnode a" rule:PCFG.induct)
       case (MainCall l p' es rets n' ins outs c)
       from `\<lambda>s. True:(Main, n')\<hookrightarrow>\<^bsub>p'\<^esub>map interpret es = kind a` `kind a = Q:r\<hookrightarrow>\<^bsub>p\<^esub>fs`
       have [simp]:"p' = p" by simp
@@ -158,7 +158,7 @@ proof -
 	  by(auto elim:PCFG.cases simp:valid_edge_def) }
       with `(p',Entry) = targetnode a` show ?case by simp
     next
-      case (ProcCall i px ins outs c l p' es rets l' ins' outs' c')
+      case (ProcCall px ins outs c l p' es rets l' ins' outs' c' ps)
       from `\<lambda>s. True:(px, Label l')\<hookrightarrow>\<^bsub>p'\<^esub>map interpret es = kind a` `kind a = Q:r\<hookrightarrow>\<^bsub>p\<^esub>fs`
       have [simp]:"p' = p" by simp
       { fix a' assume "valid_edge wfp a'" and "targetnode a' = (p', Entry)"
@@ -174,7 +174,7 @@ proof -
     from this `kind a = Q'\<hookleftarrow>\<^bsub>p\<^esub>f'`
     show "\<forall>a'. valid_edge wfp a' \<and> sourcenode a' = sourcenode a \<longrightarrow>
       (\<exists>Qx fx. kind a' = Qx\<hookleftarrow>\<^bsub>p\<^esub>fx)"
-    proof(induct n\<equiv>"sourcenode a" et\<equiv>"kind a" n'\<equiv>"targetnode a" rule:PCFG.induct)
+    proof(induct "sourcenode a" "kind a" "targetnode a" rule:PCFG.induct)
       case (MainReturn l p' es rets l' ins outs c)
       from `\<lambda>cf. snd cf = (Main, Label l')\<hookleftarrow>\<^bsub>p'\<^esub>\<lambda>cf cf'. cf'(rets [:=] map cf outs) =
 	kind a` `kind a = Q'\<hookleftarrow>\<^bsub>p\<^esub>f'` have [simp]:"p' = p" by simp
@@ -183,7 +183,7 @@ proof -
 	  by(auto elim:PCFG.cases simp:valid_edge_def) }
       with `(p', Exit) = sourcenode a` show ?case by simp
     next
-      case (ProcReturn i px ins outs c l p' es rets l' ins' outs' c')
+      case (ProcReturn px ins outs c l p' es rets l' ins' outs' c' ps)
       from `\<lambda>cf. snd cf = (px, Label l')\<hookleftarrow>\<^bsub>p'\<^esub>\<lambda>cf cf'. cf'(rets [:=] map cf outs') =
 	kind a` `kind a = Q'\<hookleftarrow>\<^bsub>p\<^esub>f'` have [simp]:"p' = p" by simp
       { fix a' assume "valid_edge wfp a'" and "sourcenode a' = (p', Exit)"
@@ -218,15 +218,16 @@ proof -
     from this `kind a = Q'\<hookleftarrow>\<^bsub>p\<^esub>f'`
     show "\<exists>!a'. valid_edge wfp a' \<and> (\<exists>Q r fs. kind a' = Q:r\<hookrightarrow>\<^bsub>p\<^esub>fs) \<and>
       a \<in> get_return_edges wfp a'"
-    proof(induct n\<equiv>"sourcenode a" et\<equiv>"kind a" n'\<equiv>"targetnode a" rule:PCFG.induct)
+    proof(induct "sourcenode a" "kind a" "targetnode a" rule:PCFG.induct)
       case (MainReturn l px es rets l' ins outs c)
       from `\<lambda>cf. snd cf = (Main, Label l')\<hookleftarrow>\<^bsub>px\<^esub>\<lambda>cf cf'. cf'(rets [:=] map cf outs) =
 	kind a` `kind a = Q'\<hookleftarrow>\<^bsub>p\<^esub>f'` have [simp]:"px = p" by simp
       from `prog \<turnstile> Label l -CEdge (px, es, rets)\<rightarrow>\<^isub>p Label l'` have "l' = Suc l"
 	by(fastsimp dest:Proc_CFG_Call_Labels)
       from `prog \<turnstile> Label l -CEdge (px, es, rets)\<rightarrow>\<^isub>p Label l'`
-	`(px, ins, outs, c) \<in> set procs`	 `distinct rets` `length rets = length outs`
-	`length es = length ins`
+      have "containsCall procs prog [] px" by(rule Proc_CFG_Call_containsCall)
+      with `prog \<turnstile> Label l -CEdge (px, es, rets)\<rightarrow>\<^isub>p Label l'`
+	`(px, ins, outs, c) \<in> set procs`	
       have "prog,procs \<turnstile> (p,Exit) -(\<lambda>cf. snd cf = (Main,Label l'))\<hookleftarrow>\<^bsub>p\<^esub>
 	(\<lambda>cf cf'. cf'(rets [:=] map cf outs))\<rightarrow> (Main,Label l')"
 	by(fastsimp intro:PCFG.MainReturn)
@@ -235,8 +236,7 @@ proof -
 	kind a`
       have edge:"prog,procs \<turnstile> sourcenode a -kind a\<rightarrow> targetnode a" by simp
       from `prog \<turnstile> Label l -CEdge (px, es, rets)\<rightarrow>\<^isub>p Label l'`
-	`(px, ins, outs, c) \<in> set procs` `distinct rets` `length rets = length outs`
-	`length es = length ins`
+	`(px, ins, outs, c) \<in> set procs`
       have edge':"prog,procs \<turnstile> (Main,Label l) 
         -(\<lambda>s. True):(Main,Label l')\<hookrightarrow>\<^bsub>p\<^esub>map (\<lambda>e cf. interpret e cf) es\<rightarrow> (p,Entry)"
 	by(fastsimp intro:MainCall)
@@ -273,32 +273,30 @@ proof -
 	with nodes nodes' show "a' = a''" by(cases a',cases a'',auto)
       qed
     next
-      case (ProcReturn i p' ins outs c l px esx retsx l' ins' outs' c' ps es rets)
+      case (ProcReturn p' ins outs c l px esx retsx l' ins' outs' c' ps)
       from `\<lambda>cf. snd cf = (p', Label l')\<hookleftarrow>\<^bsub>px\<^esub>\<lambda>cf cf'. cf'(retsx [:=] map cf outs') =
 	kind a` `kind a = Q'\<hookleftarrow>\<^bsub>p\<^esub>f'` have [simp]:"px = p" by simp
       from `c \<turnstile> Label l -CEdge (px, esx, retsx)\<rightarrow>\<^isub>p Label l'` have "l' = Suc l"
 	by(fastsimp dest:Proc_CFG_Call_Labels)
-      from `i < length procs` `procs ! i = (p',ins,outs,c)`
+      from `(p',ins,outs,c) \<in> set procs`
 	`c \<turnstile> Label l -CEdge (px, esx, retsx)\<rightarrow>\<^isub>p Label l'` 
-	`(px, ins', outs', c') \<in> set procs` `containsCall procs prog ps p' es rets`
-	`distinct retsx` `length retsx = length outs'` `length esx = length ins'`
+	`(px, ins', outs', c') \<in> set procs` `containsCall procs prog ps p'`
       have "prog,procs \<turnstile> (p,Exit) -(\<lambda>cf. snd cf = (p',Label l'))\<hookleftarrow>\<^bsub>p\<^esub>
 	(\<lambda>cf cf'. cf'(retsx [:=] map cf outs'))\<rightarrow> (p',Label l')"
 	by(fastsimp intro:PCFG.ProcReturn)
       with `(px, Exit) = sourcenode a` `(p', Label l') = targetnode a`
 	`\<lambda>cf. snd cf = (p', Label l')\<hookleftarrow>\<^bsub>px\<^esub>\<lambda>cf cf'. cf'(retsx [:=] map cf outs') =
 	kind a` have edge:"prog,procs \<turnstile> sourcenode a -kind a\<rightarrow> targetnode a" by simp
-      from `i < length procs` `procs ! i = (p',ins,outs,c)`
+      from `(p',ins,outs,c) \<in> set procs`
 	`c \<turnstile> Label l -CEdge (px, esx, retsx)\<rightarrow>\<^isub>p Label l'`
-	`(px, ins', outs', c') \<in> set procs` `containsCall procs prog ps p' es rets`
-	`distinct retsx` `length retsx = length outs'` `length esx = length ins'`
+	`(px, ins', outs', c') \<in> set procs` `containsCall procs prog ps p'`
       have edge':"prog,procs \<turnstile> (p',Label l) 
 	-(\<lambda>s. True):(p',Label l')\<hookrightarrow>\<^bsub>p\<^esub>map (\<lambda>e cf. interpret e cf) esx\<rightarrow> (p,Entry)"
 	by(fastsimp intro:ProcCall)
       show ?case
       proof(rule ex_ex1I)
 	from edge edge' `(p', Label l') = targetnode a` `l' = Suc l`
-	  `procs ! i = (p', ins, outs, c)` `i < length procs` `kind a = Q'\<hookleftarrow>\<^bsub>p\<^esub>f'`
+	  `(p', ins, outs, c) \<in> set procs` `kind a = Q'\<hookleftarrow>\<^bsub>p\<^esub>f'`
 	show "\<exists>a'. valid_edge wfp a' \<and>
           (\<exists>Q r fs. kind a' = Q:r\<hookrightarrow>\<^bsub>p\<^esub>fs) \<and> a \<in> get_return_edges wfp a'"
 	  by(fastsimp simp:valid_edge_def get_return_edges_def)
@@ -314,13 +312,13 @@ proof -
 	  and "a \<in> get_return_edges wfp a''" by blast
 	from `valid_edge wfp a'` `kind a' = Q:r\<hookrightarrow>\<^bsub>p\<^esub>fs`[THEN sym] 
 	  `a \<in> get_return_edges wfp a'` edge `(p', Label l') = targetnode a` wf
-	  `i < length procs` `procs ! i = (p', ins, outs, c)` `l' = Suc l`
+	  `(p', ins, outs, c) \<in> set procs` `l' = Suc l`
 	have nodes:"sourcenode a' = (p',Label l) \<and> targetnode a' = (p,Entry)"
 	  apply(auto simp:valid_edge_def get_return_edges_def)
 	  by(erule PCFG.cases,auto dest:Proc_CFG_Call_Labels)+
 	from `valid_edge wfp a''` `kind a'' = Q':r'\<hookrightarrow>\<^bsub>p\<^esub>fs'`[THEN sym] 
 	  `a \<in> get_return_edges wfp a''` edge `(p', Label l') = targetnode a` wf
-	  `i < length procs` `procs ! i = (p', ins, outs, c)` `l' = Suc l`
+	  `(p', ins, outs, c) \<in> set procs` `l' = Suc l`
 	have nodes':"sourcenode a'' = (p',Label l) \<and> targetnode a'' = (p,Entry)"
 	  apply(auto simp:valid_edge_def get_return_edges_def)
 	  by(erule PCFG.cases,auto dest:Proc_CFG_Call_Labels)+
@@ -351,21 +349,19 @@ proof -
       have "c \<turnstile> Entry -IEdge (\<lambda>s. False)\<^isub>\<surd>\<rightarrow>\<^isub>p Exit" by(rule Proc_CFG_Entry_Exit)
       moreover
       from `prog \<turnstile> Label l -CEdge (p, es, rets)\<rightarrow>\<^isub>p n'`
-      have "containsCall procs prog [] p es rets" by(rule Proc_CFG_Call_containsCall)
+      have "containsCall procs prog [] p" by(rule Proc_CFG_Call_containsCall)
       ultimately have "prog,procs \<turnstile> (p,Entry) -(\<lambda>s. False)\<^isub>\<surd>\<rightarrow> (p,Exit)"
 	using `(p, ins, outs, c) \<in> set procs` by(fastsimp intro:Proc)
       with `sourcenode a' = (p,Exit)` `(p, Entry) = targetnode a`[THEN sym]
       show ?case by(fastsimp simp:valid_edge_def)
     next
-      case (ProcCall i px ins outs c l es' rets' l' ins' outs' c' ps es rets)
-      from `procs ! i = (px, ins, outs, c)` `i < length procs`
-      have "(px,ins,outs,c) \<in> set procs" by(fastsimp simp:in_set_conv_nth)
+      case (ProcCall px ins outs c l es' rets' l' ins' outs' c' ps)
       have "c' \<turnstile> Entry -IEdge (\<lambda>s. False)\<^isub>\<surd>\<rightarrow>\<^isub>p Exit" by(rule Proc_CFG_Entry_Exit)
       moreover
       from `c \<turnstile> Label l -CEdge (p, es', rets')\<rightarrow>\<^isub>p Label l'`
-      have "containsCall procs c [] p es' rets'" by(rule Proc_CFG_Call_containsCall)
-      with `containsCall procs prog ps px es rets` `(px,ins,outs,c) \<in> set procs`
-      have "containsCall procs prog (ps@[px]) p es' rets'"
+      have "containsCall procs c [] p" by(rule Proc_CFG_Call_containsCall)
+      with `containsCall procs prog ps px` `(px,ins,outs,c) \<in> set procs`
+      have "containsCall procs prog (ps@[px]) p"
 	by(rule containsCall_in_proc)
       ultimately have "prog,procs \<turnstile> (p,Entry) -(\<lambda>s. False)\<^isub>\<surd>\<rightarrow> (p,Exit)"
 	using `(p, ins', outs', c') \<in> set procs` by(fastsimp intro:Proc)
@@ -388,18 +384,16 @@ proof -
       targetnode a'' = targetnode a' \<and> kind a'' = (\<lambda>cf. False)\<^isub>\<surd>"
     proof(induct "sourcenode a" "Q:r\<hookrightarrow>\<^bsub>p\<^esub>fs" "targetnode a" rule:PCFG.induct)
       case (MainCall l es rets n' ins outs c)
-      from `prog \<turnstile> Label l -CEdge (p, es, rets)\<rightarrow>\<^isub>p n'` `distinct rets`
+      from `prog \<turnstile> Label l -CEdge (p, es, rets)\<rightarrow>\<^isub>p n'`
       have "prog,procs \<turnstile> (Main,Label l) -(\<lambda>s. False)\<^isub>\<surd>\<rightarrow> (Main,n')"
 	by(rule MainCallReturn)
       with `(Main, Label l) = sourcenode a`[THEN sym] `targetnode a' = r`
         `(Main, n') = r`[THEN sym]
       show ?case by(auto simp:valid_edge_def)
     next
-      case (ProcCall i px ins outs c l es' rets' l' ins' outs' c' ps es rets)
-      from `i < length procs` `procs ! i = (px, ins, outs, c)`
-      have "(px,ins,outs,c) \<in> set procs" by(fastsimp simp:in_set_conv_nth)
-      with `c \<turnstile> Label l -CEdge (p, es', rets')\<rightarrow>\<^isub>p Label l'` `distinct rets'`
-	`containsCall procs prog ps px es rets`
+      case (ProcCall px ins outs c l es' rets' l' ins' outs' c' ps)
+      from `(px,ins,outs,c) \<in> set procs`	 `containsCall procs prog ps px`
+        `c \<turnstile> Label l -CEdge (p, es', rets')\<rightarrow>\<^isub>p Label l'`
       have "prog,procs \<turnstile> (px,Label l) -(\<lambda>s. False)\<^isub>\<surd>\<rightarrow> (px,Label l')"
 	by(fastsimp intro:ProcCallReturn)
       with `(px, Label l) = sourcenode a`[THEN sym] `targetnode a' = r`
@@ -414,11 +408,11 @@ proof -
     from this `kind a = Q:r\<hookrightarrow>\<^bsub>p\<^esub>fs` 
     show "\<exists>!a'. valid_edge wfp a' \<and>
       sourcenode a' = sourcenode a \<and> intra_kind (kind a')"
-    proof(induct n\<equiv>"sourcenode a" et\<equiv>"kind a" n'\<equiv>"targetnode a" rule:PCFG.induct)
+    proof(induct "sourcenode a" "kind a" "targetnode a" rule:PCFG.induct)
       case (MainCall l p' es rets n' ins outs c)
       show ?thesis 
       proof(rule ex_ex1I)
-	from `prog \<turnstile> Label l -CEdge (p', es, rets)\<rightarrow>\<^isub>p n'` `distinct rets`
+	from `prog \<turnstile> Label l -CEdge (p', es, rets)\<rightarrow>\<^isub>p n'`
 	have "prog,procs \<turnstile> (Main,Label l) -(\<lambda>s. False)\<^isub>\<surd>\<rightarrow> (Main,n')"
 	  by(rule MainCallReturn)
 	with `(Main, Label l) = sourcenode a`[THEN sym]
@@ -452,13 +446,11 @@ proof -
 	(auto dest:Proc_CFG_edge_det simp:valid_edge_def)
       qed
     next
-      case (ProcCall i px ins outs c l p' es' rets' l' ins' outs' c' ps esx retsx)
+      case (ProcCall px ins outs c l p' es' rets' l' ins' outs' c' ps)
       show ?thesis 
       proof(rule ex_ex1I)
-	from `i < length procs` `procs ! i = (px, ins, outs, c)`[THEN sym]
-	have "(px, ins, outs, c) \<in> set procs" by(fastsimp simp:set_conv_nth)
-	with `containsCall procs prog ps px esx retsx`
-	  `c \<turnstile> Label l -CEdge (p', es', rets')\<rightarrow>\<^isub>p Label l'` `distinct rets'`
+	from `(px, ins, outs, c) \<in> set procs` `containsCall procs prog ps px`
+	  `c \<turnstile> Label l -CEdge (p', es', rets')\<rightarrow>\<^isub>p Label l'`
 	have "prog,procs \<turnstile> (px,Label l) -(\<lambda>s. False)\<^isub>\<surd>\<rightarrow> (px,Label l')"
 	  by -(rule ProcCallReturn)
 	with `(px, Label l) = sourcenode a`[THEN sym]
@@ -474,20 +466,19 @@ proof -
 	  and "intra_kind (kind a')" and "valid_edge wfp a''"
 	  and "sourcenode a'' = sourcenode a" and "intra_kind (kind a'')" by simp_all
 	from `valid_edge wfp a'` `sourcenode a' = sourcenode a`
-	  `intra_kind (kind a')` `i < length procs` `procs ! i = (px, ins, outs, c)`
+	  `intra_kind (kind a')` `(px, ins, outs, c) \<in> set procs`
 	  `c \<turnstile> Label l -CEdge (p', es', rets')\<rightarrow>\<^isub>p Label l'`
 	  `(p', ins', outs', c') \<in> set procs` wf
-	  `containsCall procs prog ps px esx retsx` `(px, Label l) = sourcenode a`
+	  `containsCall procs prog ps px` `(px, Label l) = sourcenode a`
 	have "targetnode a' = (px,Label (Suc l))"
 	  apply(auto simp:valid_edge_def) apply(erule PCFG.cases)
 	  by(auto dest:Proc_CFG_Call_Intra_edge_not_same_source 
 	    Proc_CFG_Call_nodes_eq Proc_CFG_Call_Labels simp:intra_kind_def)
 	from `valid_edge wfp a''` `sourcenode a'' = sourcenode a`
-	  `intra_kind (kind a'')` `i < length procs`
-	  `procs ! i = (px, ins, outs, c)`
+	  `intra_kind (kind a'')` `(px, ins, outs, c) \<in> set procs`
 	  `c \<turnstile> Label l -CEdge (p', es', rets')\<rightarrow>\<^isub>p Label l'`
 	  `(p', ins', outs', c') \<in> set procs` wf
-	  `containsCall procs prog ps px esx retsx` `(px, Label l) = sourcenode a`
+	  `containsCall procs prog ps px` `(px, Label l) = sourcenode a`
 	have "targetnode a'' = (px,Label (Suc l))"
 	  apply(auto simp:valid_edge_def) apply(erule PCFG.cases)
 	  by(auto dest:Proc_CFG_Call_Intra_edge_not_same_source 
@@ -507,11 +498,11 @@ proof -
     from this `kind a = Q'\<hookleftarrow>\<^bsub>p\<^esub>f'`
     show "\<exists>!a'. valid_edge wfp a' \<and>
       targetnode a' = targetnode a \<and> intra_kind (kind a')"
-    proof(induct n\<equiv>"sourcenode a" et\<equiv>"kind a" n'\<equiv>"targetnode a" rule:PCFG.induct)
+    proof(induct "sourcenode a" "kind a" "targetnode a" rule:PCFG.induct)
       case (MainReturn l p' es rets l' ins outs c)
       show ?thesis 
       proof(rule ex_ex1I)
-	from `prog \<turnstile> Label l -CEdge (p', es, rets)\<rightarrow>\<^isub>p Label l'` `distinct rets`
+	from `prog \<turnstile> Label l -CEdge (p', es, rets)\<rightarrow>\<^isub>p Label l'`
 	have "prog,procs \<turnstile> (Main,Label l) -(\<lambda>s. False)\<^isub>\<surd>\<rightarrow> 
 	  (Main,Label l')" by(rule MainCallReturn)
 	with `(Main, Label l') = targetnode a`[THEN sym]
@@ -547,13 +538,11 @@ proof -
 	(auto dest:Proc_CFG_edge_det simp:valid_edge_def)
       qed
     next
-      case (ProcReturn i px ins outs c l p' es' rets' l' ins' outs' c' ps esx retsx)
+      case (ProcReturn px ins outs c l p' es' rets' l' ins' outs' c' ps)
       show ?thesis 
       proof(rule ex_ex1I)
-	from `i < length procs` `procs ! i = (px, ins, outs, c)`[THEN sym]
-	have "(px, ins, outs, c) \<in> set procs" by(fastsimp simp:set_conv_nth)
-	with `c \<turnstile> Label l -CEdge (p', es', rets')\<rightarrow>\<^isub>p Label l'`
-	  `distinct rets'` `containsCall procs prog ps px esx retsx`
+	from `(px, ins, outs, c) \<in> set procs` `containsCall procs prog ps px`
+          `c \<turnstile> Label l -CEdge (p', es', rets')\<rightarrow>\<^isub>p Label l'`
 	have "prog,procs \<turnstile> (px,Label l) -(\<lambda>s. False)\<^isub>\<surd>\<rightarrow> (px,Label l')"
 	  by -(rule ProcCallReturn)
 	with `(px, Label l') = targetnode a`[THEN sym]
@@ -569,19 +558,19 @@ proof -
 	  and "intra_kind (kind a')" and "valid_edge wfp a''"
 	  and "targetnode a'' = targetnode a" and "intra_kind (kind a'')" by simp_all
 	from `valid_edge wfp a'` `targetnode a' = targetnode a`
-	  `intra_kind (kind a')` `i < length procs`
-	  `procs ! i = (px, ins, outs, c)` `(p', ins', outs', c') \<in> set procs` wf
+	  `intra_kind (kind a')` `(px, ins, outs, c) \<in> set procs`
+          `(p', ins', outs', c') \<in> set procs` wf
 	  `c \<turnstile> Label l -CEdge (p', es', rets')\<rightarrow>\<^isub>p Label l'`
-	  `containsCall procs prog ps px esx retsx` `(px, Label l') = targetnode a`
+	  `containsCall procs prog ps px` `(px, Label l') = targetnode a`
 	have "sourcenode a' = (px,Label l)"
 	  apply(auto simp:valid_edge_def) apply(erule PCFG.cases)
 	  by(auto dest:Proc_CFG_Call_Intra_edge_not_same_target 
 	    Proc_CFG_Call_nodes_eq' simp:intra_kind_def)
 	from `valid_edge wfp a''` `targetnode a'' = targetnode a`
-	  `intra_kind (kind a'')` `i < length procs`
-	  `procs ! i = (px, ins, outs, c)` `(p', ins', outs', c') \<in> set procs` wf
+	  `intra_kind (kind a'')` `(px, ins, outs, c) \<in> set procs`
+          `(p', ins', outs', c') \<in> set procs` wf
 	  `c \<turnstile> Label l -CEdge (p', es', rets')\<rightarrow>\<^isub>p Label l'`
-	  `containsCall procs prog ps px esx retsx` `(px, Label l') = targetnode a`
+	  `containsCall procs prog ps px` `(px, Label l') = targetnode a`
 	have "sourcenode a'' = (px,Label l)"
 	  apply(auto simp:valid_edge_def) apply(erule PCFG.cases)
 	  by(auto dest:Proc_CFG_Call_Intra_edge_not_same_target 
