thys/HRB-Slicing/Proc/ValidPaths.thy
@@ -22,7 +22,7 @@ subsubsection {* From @{text prog} to @{text "prog;;c\<^isub>2"} *}
 
 lemma Proc_CFG_edge_SeqFirst_nodes_Label:
   "prog \<turnstile> Label l -et\<rightarrow>\<^isub>p Label l' \<Longrightarrow> prog;;c\<^isub>2 \<turnstile> Label l -et\<rightarrow>\<^isub>p Label l'"
-proof(induct prog n\<equiv>"Label l" et n'\<equiv>"Label l'" rule:Proc_CFG.induct)
+proof(induct prog "Label l" et "Label l'" rule:Proc_CFG.induct)
   case (Proc_CFG_SeqSecond c\<^isub>2' n et n' c\<^isub>1)
   hence "(c\<^isub>1;; c\<^isub>2');; c\<^isub>2 \<turnstile> n \<oplus> #:c\<^isub>1 -et\<rightarrow>\<^isub>p n' \<oplus> #:c\<^isub>1"
     by(fastsimp intro:Proc_CFG_SeqFirst Proc_CFG.Proc_CFG_SeqSecond)
@@ -152,33 +152,33 @@ proof(atomize_elim)
     with `Main = p` `Main = p'` show ?case 
       by(fastsimp dest:PCFG.Main)
   next
-    case (Proc ins outs c et ps es rets)
-    from `containsCall procs prog ps p es rets` 
-    have "containsCall procs (prog;;c\<^isub>2) ps p es rets" by simp
+    case (Proc ins outs c et ps)
+    from `containsCall procs prog ps p`
+    have "containsCall procs (prog;;c\<^isub>2) ps p" by simp
     with Proc show ?case by(fastsimp dest:PCFG.Proc)
   next
     case (MainCall es rets nx ins outs c)
     from `prog \<turnstile> Label l -CEdge (p', es, rets)\<rightarrow>\<^isub>p nx`
-    obtain lx' where [simp]:"nx = Label lx'" by(fastsimp dest:Proc_CFG_Call_Labels)
+    obtain lx where [simp]:"nx = Label lx" by(fastsimp dest:Proc_CFG_Call_Labels)
     with `prog \<turnstile> Label l -CEdge (p', es, rets)\<rightarrow>\<^isub>p nx`
-    have "prog;;c\<^isub>2 \<turnstile> Label l -CEdge (p', es, rets)\<rightarrow>\<^isub>p Label lx'"
+    have "prog;;c\<^isub>2 \<turnstile> Label l -CEdge (p', es, rets)\<rightarrow>\<^isub>p Label lx"
       by(auto intro:Proc_CFG_edge_SeqFirst_nodes_Label)
     with MainCall show ?case by(fastsimp dest:PCFG.MainCall)
   next
-    case (ProcCall i ins outs c es' rets' l' ins' outs' c' ps es rets)
-    from `containsCall procs prog ps p es rets` 
-    have "containsCall procs (prog;;c\<^isub>2) ps p es rets" by simp
-    with ProcCall show ?case by(fastsimp dest!:PCFG.ProcCall)
+    case (ProcCall ins outs c es' rets' l' ins' outs' c' ps)
+    from `containsCall procs prog ps p` 
+    have "containsCall procs (prog;;c\<^isub>2) ps p" by simp
+    with ProcCall show ?case by(fastsimp intro:PCFG.ProcCall)
   next
     case (MainCallReturn px es rets)
-    from `prog \<turnstile> Label l -CEdge (px, es, rets)\<rightarrow>\<^isub>p n'`
+    from `prog \<turnstile> Label l -CEdge (px, es, rets)\<rightarrow>\<^isub>p n'` `Main = p`
     obtain nx'' where "prog;;c\<^isub>2 \<turnstile> Label l -CEdge (px, es, rets)\<rightarrow>\<^isub>p nx''"
       by(auto elim:Proc_CFG_edge_SeqFirst_source_Label)
     with MainCallReturn show ?case by(fastsimp dest:PCFG.MainCallReturn)
   next
-    case (ProcCallReturn ins outs c px' es' rets' ps es rets)
-    from `containsCall procs prog ps p es rets`
-    have "containsCall procs (prog;;c\<^isub>2) ps p es rets" by simp
+    case (ProcCallReturn ins outs c px' es' rets' ps)
+    from `containsCall procs prog ps p`
+    have "containsCall procs (prog;;c\<^isub>2) ps p" by simp
     with ProcCallReturn show ?case by(fastsimp dest!:PCFG.ProcCallReturn)
   qed
 qed
@@ -191,26 +191,26 @@ proof(induct "(p,n)" et "(p',Label l')" rule:PCFG.induct)
   case Main
   thus ?case by(fastsimp dest:Proc_CFG_edge_SeqFirst_target_Label intro:PCFG.Main)
 next
-  case (Proc ins outs c et ps es rets)
-  from `containsCall procs prog ps p es rets` 
-  have "containsCall procs (prog;;c\<^isub>2) ps p es rets" by simp
+  case (Proc ins outs c et ps)
+  from `containsCall procs prog ps p` 
+  have "containsCall procs (prog;;c\<^isub>2) ps p" by simp
   with Proc show ?case by(fastsimp dest:PCFG.Proc)
 next
   case MainReturn thus ?case
     by(fastsimp dest:Proc_CFG_edge_SeqFirst_target_Label 
                intro!:PCFG.MainReturn[simplified])
 next
-  case (ProcReturn i ins outs c lx es' rets' ins' outs' c' ps es rets)
-  from `containsCall procs prog ps p' es rets`
-  have "containsCall procs (prog;;c\<^isub>2) ps p' es rets" by simp
-  with ProcReturn show ?case by(fastsimp dest!:PCFG.ProcReturn)
+  case (ProcReturn ins outs c lx es' rets' ins' outs' c' ps)
+  from `containsCall procs prog ps p'` 
+  have "containsCall procs (prog;;c\<^isub>2) ps p'" by simp
+  with ProcReturn show ?case by(fastsimp intro:PCFG.ProcReturn)
 next
   case MainCallReturn thus ?case
   by(fastsimp dest:Proc_CFG_edge_SeqFirst_target_Label intro:PCFG.MainCallReturn)
 next
-  case (ProcCallReturn ins outs c px' es' rets' ps es rets)
-  from `containsCall procs prog ps p es rets` 
-  have "containsCall procs (prog;;c\<^isub>2) ps p es rets" by simp
+  case (ProcCallReturn ins outs c px' es' rets' ps)
+  from `containsCall procs prog ps p` 
+  have "containsCall procs (prog;;c\<^isub>2) ps p" by simp
   with ProcCallReturn show ?case by(fastsimp dest!:PCFG.ProcCallReturn)
 qed
 
@@ -221,17 +221,15 @@ lemma path_SeqFirst:
   \<Longrightarrow> wfp' \<turnstile> (p,n) -as\<rightarrow>* (p,Label l)"
 proof(induct "(p,n)" as "(p,Label l)" arbitrary:n rule:ProcCFG.path.induct)
   case empty_path
-  from `CFG.valid_node sourcenode targetnode (valid_edge wfp) (p,Label l)` 
-    `Rep_wf_prog wfp = (prog, procs)` 
-    `Rep_wf_prog wfp' = (prog;; c\<^isub>2, procs)`
-  have "CFG.valid_node sourcenode targetnode (valid_edge wfp') (p,Label l)"
+  from `CFG.valid_node sourcenode targetnode (valid_edge wfp) (p, Label l)` 
+    `Rep_wf_prog wfp = (prog, procs)` `Rep_wf_prog wfp' = (prog;; c\<^isub>2, procs)`
+  have "CFG.valid_node sourcenode targetnode (valid_edge wfp') (p, Label l)"
     apply(auto simp:ProcCFG.valid_node_def valid_edge_def)
     apply(erule PCFG_edge_SeqFirst_source_Label,fastsimp)
     by(drule PCFG_edge_SeqFirst_target_Label,fastsimp)
-  then show ?case
-    by(fastsimp intro:ProcCFG.empty_path)
+  thus ?case by(fastsimp intro:ProcCFG.empty_path)
 next
-  case (Cons_path n'' as a)
+  case (Cons_path n'' as a nx)
   note IH = `\<And>n. \<lbrakk>n'' = (p, n); \<forall>a\<in>set as. intra_kind (kind a)\<rbrakk>
     \<Longrightarrow> wfp' \<turnstile> (p, n) -as\<rightarrow>* (p, Label l)`
   note [simp] = `Rep_wf_prog wfp = (prog,procs)` `Rep_wf_prog wfp' = (prog;;c\<^isub>2,procs)`
@@ -239,7 +237,7 @@ next
     by(fastsimp intro:wf_wf_prog)
   from `\<forall>a\<in>set (a # as). intra_kind (kind a)` have "intra_kind (kind a)"
     and "\<forall>a\<in>set as. intra_kind (kind a)" by simp_all
-  from `valid_edge wfp a` `sourcenode a = (p, n)` `targetnode a = n''`
+  from `valid_edge wfp a` `sourcenode a = (p, nx)` `targetnode a = n''`
     `intra_kind (kind a)` wf 
   obtain nx' where "n'' = (p,nx')"
     by(auto elim:PCFG.cases simp:valid_edge_def intra_kind_def)
@@ -248,7 +246,7 @@ next
   have "valid_edge wfp' a"
   proof(cases nx')
     case (Label lx)
-    with `valid_edge wfp a` `sourcenode a = (p, n)` `targetnode a = n''`
+    with `valid_edge wfp a` `sourcenode a = (p, nx)` `targetnode a = n''`
       `n'' = (p,nx')` show ?thesis
       by(fastsimp intro:PCFG_edge_SeqFirst_target_Label 
 	           simp:intra_kind_def valid_edge_def)
@@ -261,11 +259,11 @@ next
   next
     case Exit
     with path `\<forall>a\<in>set as. intra_kind (kind a)` have False 
-      by(induct x\<equiv>"(p,nx')" as x'\<equiv>"(p,Label l)" rule:ProcCFG.path.induct)
+      by(induct "(p,nx')" as "(p,Label l)" rule:ProcCFG.path.induct)
     (auto elim!:PCFG.cases simp:valid_edge_def intra_kind_def)
     thus ?thesis by simp
   qed
-  with `sourcenode a = (p, n)` `targetnode a = n''` `n'' = (p,nx')` path
+  with `sourcenode a = (p, nx)` `targetnode a = n''` `n'' = (p,nx')` path
   show ?case by(fastsimp intro:ProcCFG.Cons_path)
 qed
 
@@ -316,7 +314,7 @@ proof -
       from `n \<noteq> Entry` `prog \<turnstile> nx -IEdge (kind a)\<rightarrow>\<^isub>p nx'`
       have "c\<^isub>1;;prog \<turnstile> n \<oplus> #:c\<^isub>1 -IEdge (kind a)\<rightarrow>\<^isub>p nx' \<oplus> #:c\<^isub>1"
 	by(fastsimp intro:Proc_CFG_edge_SeqSecond_source_not_Entry)
-      hence "c\<^isub>1;;prog,procs \<turnstile> (Main,n \<oplus> #:c\<^isub>1) -(kind a)\<rightarrow> (Main,nx' \<oplus> #:c\<^isub>1)"
+      hence "c\<^isub>1;;prog,procs \<turnstile> (Main,n \<oplus> #:c\<^isub>1) -kind a\<rightarrow> (Main,nx' \<oplus> #:c\<^isub>1)"
 	by(rule PCFG.Main)
       thus ?thesis by(simp add:ProcCFG.valid_node_def)(fastsimp simp:valid_edge_def)
     next
@@ -349,15 +347,17 @@ proof -
 	with `prog \<turnstile> nx -IEdge (kind a)\<rightarrow>\<^isub>p nx'`
 	have "c\<^isub>1;;prog \<turnstile> nx \<oplus> #:c\<^isub>1 -IEdge (kind a)\<rightarrow>\<^isub>p nx' \<oplus> #:c\<^isub>1"
 	  by(fastsimp intro:Proc_CFG_edge_SeqSecond_source_not_Entry)
-	hence "c\<^isub>1;;prog,procs \<turnstile> (Main,nx \<oplus> #:c\<^isub>1) -(kind a)\<rightarrow> (Main,nx' \<oplus> #:c\<^isub>1)"
+	hence "c\<^isub>1;;prog,procs \<turnstile> (Main,nx \<oplus> #:c\<^isub>1) -kind a\<rightarrow> (Main,nx' \<oplus> #:c\<^isub>1)"
 	  by(rule PCFG.Main)
 	with `(Main, n) = targetnode a` `(Main, nx') = targetnode a`[THEN sym]
 	show ?thesis by(simp add:ProcCFG.valid_node_def)(fastsimp simp:valid_edge_def)
       qed
     qed
   next
-    case (Proc p ins outs c nx n' es rets)
-    from Proc(4)[THEN sym] Proc(5)[THEN sym] Proc(1-3,6-8) have False by fastsimp
+    case (Proc p ins outs c nx n' ps)
+    from `(p, nx) = sourcenode a`[THEN sym] `(p, n') = targetnode a`[THEN sym]
+      `(Main, n) = sourcenode a \<or> (Main, n) = targetnode a` 
+      `(p, ins, outs, c) \<in> set procs` `well_formed procs` have False by fastsimp
     thus ?case by simp
   next
     case (MainCall l p es rets n' ins outs c)
@@ -368,15 +368,17 @@ proof -
     from `prog \<turnstile> Label l -CEdge (p, es, rets)\<rightarrow>\<^isub>p n'`
     have "c\<^isub>1;;prog \<turnstile> Label l \<oplus> #:c\<^isub>1 -CEdge (p, es, rets)\<rightarrow>\<^isub>p n' \<oplus> #:c\<^isub>1"
       by -(rule Proc_CFG_edge_SeqSecond_source_not_Entry,auto)
-    with `(p, ins, outs, c) \<in> set procs` `distinct rets`
-      `length rets = length outs` `length es = length ins`
+    with `(p, ins, outs, c) \<in> set procs`
     have "c\<^isub>1;;prog,procs \<turnstile> (Main,Label (l + #:c\<^isub>1)) 
       -(\<lambda>s. True):(Main,n' \<oplus> #:c\<^isub>1)\<hookrightarrow>\<^bsub>p\<^esub>map (\<lambda>e cf. interpret e cf) es\<rightarrow> (p,Entry)"
       by(fastsimp intro:PCFG.MainCall)
     thus ?case by(simp add:ProcCFG.valid_node_def)(fastsimp simp:valid_edge_def)
   next
-    case (ProcCall i p ins outs c l p' es' rets' l' ins' outs' c' es rets)
-    from ProcCall(9)[THEN sym] ProcCall(11)[THEN sym] ProcCall(1-8,10,12-14)
+    case (ProcCall p ins outs c l p' es' rets' l' ins' outs' c')
+    from `(p, Label l) = sourcenode a`[THEN sym]
+      `(p', Entry) = targetnode a`[THEN sym]  `well_formed procs`
+      `(p, ins, outs, c) \<in> set procs` `(p', ins', outs', c') \<in> set procs`
+      `(Main, n) = sourcenode a \<or> (Main, n) = targetnode a`
     have False by fastsimp
     thus ?case by simp
   next
@@ -388,15 +390,17 @@ proof -
     from `prog \<turnstile> Label l -CEdge (p, es, rets)\<rightarrow>\<^isub>p Label l'`
     have "c\<^isub>1;;prog \<turnstile> Label l \<oplus> #:c\<^isub>1 -CEdge (p, es, rets)\<rightarrow>\<^isub>p Label l' \<oplus> #:c\<^isub>1"
       by -(rule Proc_CFG_edge_SeqSecond_source_not_Entry,auto)
-    with `(p, ins, outs, c) \<in> set procs` `distinct rets`
-      `length rets = length outs` `length es = length ins`
+    with `(p, ins, outs, c) \<in> set procs`
     have "c\<^isub>1;;prog,procs \<turnstile> (p,Exit) -(\<lambda>cf. snd cf = (Main,Label l' \<oplus> #:c\<^isub>1))\<hookleftarrow>\<^bsub>p\<^esub>
       (\<lambda>cf cf'. cf'(rets [:=] map cf outs))\<rightarrow> (Main,Label (l' + #:c\<^isub>1))"
       by(fastsimp intro:PCFG.MainReturn)
     thus ?case by(simp add:ProcCFG.valid_node_def)(fastsimp simp:valid_edge_def)
   next
-    case (ProcReturn i p ins outs c l p' es' rets' l' ins' outs' c' es rets)
-    from ProcReturn(9)[THEN sym] ProcReturn(11)[THEN sym] ProcReturn(1-8,10,12-14)
+    case (ProcReturn p ins outs c l p' es' rets' l' ins' outs' c' ps)
+    from `(p', Exit) = sourcenode a`[THEN sym] 
+      `(p, Label l') = targetnode a`[THEN sym] `well_formed procs`
+      `(p, ins, outs, c) \<in> set procs` `(p', ins', outs', c') \<in> set procs`
+      `(Main, n) = sourcenode a \<or> (Main, n) = targetnode a`
     have False by fastsimp
     thus ?case by simp
   next
@@ -408,8 +412,7 @@ proof -
       from `n \<noteq> Entry` `prog \<turnstile> nx -CEdge (p, es, rets)\<rightarrow>\<^isub>p nx'`
       have "c\<^isub>1;;prog \<turnstile> n \<oplus> #:c\<^isub>1 -CEdge (p, es, rets)\<rightarrow>\<^isub>p nx' \<oplus> #:c\<^isub>1"
 	by(fastsimp intro:Proc_CFG_edge_SeqSecond_source_not_Entry)
-      with `distinct rets`
-      have "c\<^isub>1;;prog,procs \<turnstile> (Main,n \<oplus> #:c\<^isub>1) -(\<lambda>s. False)\<^isub>\<surd>\<rightarrow> (Main,nx' \<oplus> #:c\<^isub>1)"
+      hence "c\<^isub>1;;prog,procs \<turnstile> (Main,n \<oplus> #:c\<^isub>1) -(\<lambda>s. False)\<^isub>\<surd>\<rightarrow> (Main,nx' \<oplus> #:c\<^isub>1)"
 	by -(rule PCFG.MainCallReturn)
       thus ?thesis by(simp add:ProcCFG.valid_node_def)(fastsimp simp:valid_edge_def)
     next
@@ -419,16 +422,17 @@ proof -
       with `prog \<turnstile> nx -CEdge (p, es, rets)\<rightarrow>\<^isub>p nx'`
       have "c\<^isub>1;;prog \<turnstile> nx \<oplus> #:c\<^isub>1 -CEdge (p, es, rets)\<rightarrow>\<^isub>p nx' \<oplus> #:c\<^isub>1"
 	by(fastsimp intro:Proc_CFG_edge_SeqSecond_source_not_Entry)
-      with `distinct rets`
-      have "c\<^isub>1;;prog,procs \<turnstile> (Main,nx \<oplus> #:c\<^isub>1) -(\<lambda>s. False)\<^isub>\<surd>\<rightarrow> (Main,nx' \<oplus> #:c\<^isub>1)"
+      hence "c\<^isub>1;;prog,procs \<turnstile> (Main,nx \<oplus> #:c\<^isub>1) -(\<lambda>s. False)\<^isub>\<surd>\<rightarrow> (Main,nx' \<oplus> #:c\<^isub>1)"
 	by -(rule PCFG.MainCallReturn)
       with `(Main, n) = targetnode a` `(Main, nx') = targetnode a`[THEN sym] 
       show ?thesis by(simp add:ProcCFG.valid_node_def)(fastsimp simp:valid_edge_def)
     qed
   next
-    case (ProcCallReturn p ins outs c nx p' es' rets' n' es rets)
-    from ProcCallReturn(5)[THEN sym] ProcCallReturn(7)[THEN sym]
-      ProcCallReturn(1-4,6,8-10) have False by fastsimp
+    case (ProcCallReturn p ins outs c nx p' es' rets' n' ps)
+    from `(p, nx) = sourcenode a`[THEN sym] `(p, n') = targetnode a`[THEN sym]
+      `(p, ins, outs, c) \<in> set procs` `well_formed procs`
+      `(Main, n) = sourcenode a \<or> (Main, n) = targetnode a`
+    have False by fastsimp
     thus ?case by simp
   qed
 qed
@@ -448,27 +452,26 @@ proof(induct "(Main,n)" as "(p',n')" arbitrary:n rule:ProcCFG.path.induct)
   with `Main = p'` show ?case
     by(fastsimp intro:ProcCFG.empty_path simp:label_incrs_def)
 next
-  case (Cons_path n'' as a nx)
-  note IH = `\<And>n. \<lbrakk>n'' = (Main, n); \<forall>a\<in>set as. intra_kind (kind a); n \<noteq> Entry\<rbrakk>
+  case (Cons_path n'' as a n)
+  note IH = `\<And>n.  \<lbrakk>n'' = (Main, n); \<forall>a\<in>set as. intra_kind (kind a); n \<noteq> Entry\<rbrakk> 
     \<Longrightarrow> wfp' \<turnstile> (Main, n \<oplus> #:c\<^isub>1) -as \<oplus>s #:c\<^isub>1\<rightarrow>* (p', n' \<oplus> #:c\<^isub>1)`
   note [simp] = `Rep_wf_prog wfp = (prog,procs)` `Rep_wf_prog wfp' = (c\<^isub>1;;prog,procs)`
   from `Rep_wf_prog wfp = (prog,procs)` have wf:"well_formed procs" 
     by(fastsimp intro:wf_wf_prog)
   from `\<forall>a\<in>set (a # as). intra_kind (kind a)` have "intra_kind (kind a)"
     and "\<forall>a\<in>set as. intra_kind (kind a)" by simp_all
-  from `valid_edge wfp a` `sourcenode a = (Main, nx)` `targetnode a = n''`
+  from `valid_edge wfp a` `sourcenode a = (Main, n)` `targetnode a = n''`
     `intra_kind (kind a)` wf 
   obtain nx'' where "n'' = (Main,nx'')" and "nx'' \<noteq> Entry"
     by(auto elim!:PCFG.cases simp:valid_edge_def intra_kind_def)
   from IH[OF `n'' = (Main,nx'')` `\<forall>a\<in>set as. intra_kind (kind a)` `nx'' \<noteq> Entry`]
   have path:"wfp' \<turnstile> (Main, nx'' \<oplus> #:c\<^isub>1) -as \<oplus>s #:c\<^isub>1\<rightarrow>* (p', n' \<oplus> #:c\<^isub>1)" .
-  from `valid_edge wfp a` `sourcenode a = (Main, nx)` `targetnode a = n''`
-    `n'' = (Main,nx'')` `nx \<noteq> Entry` `intra_kind (kind a)` wf
-  have "c\<^isub>1;; prog,procs \<turnstile> (Main, nx\<oplus>#:c\<^isub>1) -kind a\<rightarrow> (Main, nx''\<oplus>#:c\<^isub>1)"
+  from `valid_edge wfp a` `sourcenode a = (Main, n)` `targetnode a = n''`
+    `n'' = (Main,nx'')` `n \<noteq> Entry` `intra_kind (kind a)` wf
+  have "c\<^isub>1;; prog,procs \<turnstile> (Main, n \<oplus> #:c\<^isub>1) -kind a\<rightarrow> (Main, nx'' \<oplus> #:c\<^isub>1)"
     by(fastsimp intro:PCFG_Main_edge_SeqSecond_source_not_Entry simp:valid_edge_def)
-  with path `sourcenode a = (Main, nx)` `targetnode a = n''`
-    `n'' = (Main,nx'')` show ?case
-    apply(cases a) apply(clarsimp simp:label_incrs_def)
+  with path `sourcenode a = (Main, n)` `targetnode a = n''` `n'' = (Main,nx'')`
+  show ?case apply(cases a) apply(clarsimp simp:label_incrs_def)
     by(auto intro:ProcCFG.Cons_path simp:valid_edge_def)
 qed
 
@@ -519,7 +522,7 @@ proof -
       from `n \<noteq> Entry` `prog \<turnstile> nx -IEdge (kind a)\<rightarrow>\<^isub>p nx'`
       have "if (b) prog else c\<^isub>2 \<turnstile> n \<oplus> 1 -IEdge (kind a)\<rightarrow>\<^isub>p nx' \<oplus> 1"
 	by(fastsimp intro:Proc_CFG_edge_CondTrue_source_not_Entry)
-      hence "if (b) prog else c\<^isub>2,procs \<turnstile> (Main,n \<oplus> 1) -(kind a)\<rightarrow> (Main,nx' \<oplus> 1)"
+      hence "if (b) prog else c\<^isub>2,procs \<turnstile> (Main,n \<oplus> 1) -kind a\<rightarrow> (Main,nx' \<oplus> 1)"
 	by(rule PCFG.Main)
       thus ?thesis by(simp add:ProcCFG.valid_node_def)(fastsimp simp:valid_edge_def)
     next
@@ -527,7 +530,7 @@ proof -
       show ?thesis
       proof(cases "nx = Entry")
 	case True
-	with `prog \<turnstile> nx -IEdge (kind a)\<rightarrow>\<^isub>p nx'` 
+	with `prog \<turnstile> nx -IEdge (kind a)\<rightarrow>\<^isub>p nx'`
 	have "nx' = Exit \<or> nx' = Label 0" by(fastsimp dest:Proc_CFG_EntryD)
 	thus ?thesis
 	proof
@@ -552,15 +555,18 @@ proof -
 	with `prog \<turnstile> nx -IEdge (kind a)\<rightarrow>\<^isub>p nx'`
 	have "if (b) prog else c\<^isub>2 \<turnstile> nx \<oplus> 1 -IEdge (kind a)\<rightarrow>\<^isub>p nx' \<oplus> 1"
 	  by(fastsimp intro:Proc_CFG_edge_CondTrue_source_not_Entry)
-	hence "if (b) prog else c\<^isub>2,procs \<turnstile> (Main,nx \<oplus> 1) -(kind a)\<rightarrow> 
+	hence "if (b) prog else c\<^isub>2,procs \<turnstile> (Main,nx \<oplus> 1) -kind a\<rightarrow> 
 	  (Main,nx' \<oplus> 1)" by(rule PCFG.Main)
 	with `(Main, n) = targetnode a` `(Main, nx') = targetnode a`[THEN sym]
 	show ?thesis by(simp add:ProcCFG.valid_node_def)(fastsimp simp:valid_edge_def)
       qed
     qed
   next
-    case (Proc p ins outs c nx n' es rets)
-    from Proc(4)[THEN sym] Proc(5)[THEN sym] Proc(1-3,6-8) have False by fastsimp
+    case (Proc p ins outs c nx n' ps)
+    from `(p, nx) = sourcenode a`[THEN sym] `(p, n') = targetnode a`[THEN sym]
+      `(p, ins, outs, c) \<in> set procs` `well_formed procs`
+      `(Main, n) = sourcenode a \<or> (Main, n) = targetnode a`
+    have False by fastsimp
     thus ?case by simp
   next
     case (MainCall l p es rets n' ins outs c)
@@ -571,15 +577,17 @@ proof -
     from `prog \<turnstile> Label l -CEdge (p, es, rets)\<rightarrow>\<^isub>p n'`
     have "if (b) prog else c\<^isub>2 \<turnstile> Label l \<oplus> 1 -CEdge (p, es, rets)\<rightarrow>\<^isub>p n' \<oplus> 1"
       by -(rule Proc_CFG_edge_CondTrue_source_not_Entry,auto)
-    with `(p, ins, outs, c) \<in> set procs` `distinct rets`
-      `length rets = length outs` `length es = length ins`
+    with `(p, ins, outs, c) \<in> set procs`
     have "if (b) prog else c\<^isub>2,procs \<turnstile> (Main,Label (l + 1)) 
       -(\<lambda>s. True):(Main,n' \<oplus> 1)\<hookrightarrow>\<^bsub>p\<^esub>map (\<lambda>e cf. interpret e cf) es\<rightarrow> (p,Entry)"
       by(fastsimp intro:PCFG.MainCall)
     thus ?case by(simp add:ProcCFG.valid_node_def)(fastsimp simp:valid_edge_def)
   next
-    case (ProcCall i p ins outs c l p' es' rets' l' ins' outs' c' es rets)
-    from ProcCall(9)[THEN sym] ProcCall(11)[THEN sym] ProcCall(1-8,10,12-14)
+    case (ProcCall p ins outs c l p' es' rets' l' ins' outs' c' ps)
+    from `(p, Label l) = sourcenode a`[THEN sym] 
+      `(p', Entry) = targetnode a`[THEN sym] `well_formed procs` 
+      `(p, ins, outs, c) \<in> set procs` `(p', ins', outs', c') \<in> set procs`
+      `(Main, n) = sourcenode a \<or> (Main, n) = targetnode a`
     have False by fastsimp
     thus ?case by simp
   next
@@ -591,15 +599,17 @@ proof -
     from `prog \<turnstile> Label l -CEdge (p, es, rets)\<rightarrow>\<^isub>p Label l'`
     have "if (b) prog else c\<^isub>2 \<turnstile> Label l \<oplus> 1 -CEdge (p, es, rets)\<rightarrow>\<^isub>p Label l' \<oplus> 1"
       by -(rule Proc_CFG_edge_CondTrue_source_not_Entry,auto)
-    with `(p, ins, outs, c) \<in> set procs` `distinct rets`
-      `length rets = length outs` `length es = length ins`
+    with `(p, ins, outs, c) \<in> set procs`
     have "if (b) prog else c\<^isub>2,procs \<turnstile> (p,Exit) -(\<lambda>cf. snd cf = (Main,Label l' \<oplus> 1))\<hookleftarrow>\<^bsub>p\<^esub>
       (\<lambda>cf cf'. cf'(rets [:=] map cf outs))\<rightarrow> (Main,Label (l' + 1))"
       by(fastsimp intro:PCFG.MainReturn)
     thus ?case by(simp add:ProcCFG.valid_node_def)(fastsimp simp:valid_edge_def)
   next
-    case (ProcReturn i p ins outs c l p' es' rets' l' ins' outs' c' es rets)
-    from ProcReturn(9)[THEN sym] ProcReturn(11)[THEN sym] ProcReturn(1-8,10,12-14)
+    case (ProcReturn p ins outs c l p' es' rets' l' ins' outs' c' ps)
+    from `(p', Exit) = sourcenode a`[THEN sym] 
+      `(p, Label l') = targetnode a`[THEN sym] `well_formed procs`
+      `(p, ins, outs, c) \<in> set procs` `(p', ins', outs', c') \<in> set procs`
+      `(Main, n) = sourcenode a \<or> (Main, n) = targetnode a`
     have False by fastsimp
     thus ?case by simp
   next
@@ -611,8 +621,7 @@ proof -
       from `n \<noteq> Entry` `prog \<turnstile> nx -CEdge (p, es, rets)\<rightarrow>\<^isub>p nx'`
       have "if (b) prog else c\<^isub>2 \<turnstile> n \<oplus> 1 -CEdge (p, es, rets)\<rightarrow>\<^isub>p nx' \<oplus> 1"
 	by(fastsimp intro:Proc_CFG_edge_CondTrue_source_not_Entry)
-      with `distinct rets`
-      have "if (b) prog else c\<^isub>2,procs \<turnstile> (Main,n \<oplus> 1) -(\<lambda>s. False)\<^isub>\<surd>\<rightarrow> 
+      hence "if (b) prog else c\<^isub>2,procs \<turnstile> (Main,n \<oplus> 1) -(\<lambda>s. False)\<^isub>\<surd>\<rightarrow> 
 	(Main,nx' \<oplus> 1)" by -(rule PCFG.MainCallReturn)
       thus ?thesis by(simp add:ProcCFG.valid_node_def)(fastsimp simp:valid_edge_def)
     next
@@ -622,16 +631,17 @@ proof -
       with `prog \<turnstile> nx -CEdge (p, es, rets)\<rightarrow>\<^isub>p nx'`
       have "if (b) prog else c\<^isub>2 \<turnstile> nx \<oplus> 1 -CEdge (p, es, rets)\<rightarrow>\<^isub>p nx' \<oplus> 1"
 	by(fastsimp intro:Proc_CFG_edge_CondTrue_source_not_Entry)
-      with `distinct rets`
-      have "if (b) prog else c\<^isub>2,procs \<turnstile> (Main,nx \<oplus> 1) -(\<lambda>s. False)\<^isub>\<surd>\<rightarrow> (Main,nx' \<oplus> 1)"
+      hence "if (b) prog else c\<^isub>2,procs \<turnstile> (Main,nx \<oplus> 1) -(\<lambda>s. False)\<^isub>\<surd>\<rightarrow> (Main,nx' \<oplus> 1)"
 	by -(rule PCFG.MainCallReturn)
       with `(Main, n) = targetnode a` `(Main, nx') = targetnode a`[THEN sym]
       show ?thesis by(simp add:ProcCFG.valid_node_def)(fastsimp simp:valid_edge_def)
     qed
   next
-    case (ProcCallReturn p ins outs c nx p' es' rets' n' es rets)
-    from ProcCallReturn(5)[THEN sym] ProcCallReturn(7)[THEN sym]
-      ProcCallReturn(1-4,6,8-10) have False by fastsimp
+    case (ProcCallReturn p ins outs c nx p' es' rets' n' ps)
+    from `(p, nx) = sourcenode a`[THEN sym] `(p, n') = targetnode a`[THEN sym]
+      `(p, ins, outs, c) \<in> set procs` `well_formed procs`
+      `(Main, n) = sourcenode a \<or> (Main, n) = targetnode a`
+    have False by fastsimp
     thus ?case by simp
   qed
 qed
@@ -652,8 +662,8 @@ proof(induct "(Main,n)" as "(p',n')" arbitrary:n rule:ProcCFG.path.induct)
   with `Main = p'` show ?case
     by(fastsimp intro:ProcCFG.empty_path simp:label_incrs_def)
 next
-  case (Cons_path n'' as a nx)
-  note IH = `\<And>n.  \<lbrakk>n'' = (Main, n); \<forall>a\<in>set as. intra_kind (kind a); n \<noteq> Entry\<rbrakk>
+  case (Cons_path n'' as a n)
+  note IH = `\<And>n.  \<lbrakk>n'' = (Main, n); \<forall>a\<in>set as. intra_kind (kind a); n \<noteq> Entry\<rbrakk> 
     \<Longrightarrow> wfp' \<turnstile> (Main, n \<oplus> 1) -as \<oplus>s 1\<rightarrow>* (p', n' \<oplus> 1)`
   note [simp] = `Rep_wf_prog wfp = (prog,procs)` 
     `Rep_wf_prog wfp' = (if (b) prog else c\<^isub>2,procs)`
@@ -661,18 +671,18 @@ next
     by(fastsimp intro:wf_wf_prog)
   from `\<forall>a\<in>set (a # as). intra_kind (kind a)` have "intra_kind (kind a)"
     and "\<forall>a\<in>set as. intra_kind (kind a)" by simp_all
-  from `valid_edge wfp a` `sourcenode a = (Main, nx)` `targetnode a = n''`
+  from `valid_edge wfp a` `sourcenode a = (Main, n)` `targetnode a = n''`
     `intra_kind (kind a)` wf 
   obtain nx'' where "n'' = (Main,nx'')" and "nx'' \<noteq> Entry"
     by(auto elim!:PCFG.cases simp:valid_edge_def intra_kind_def)
   from IH[OF `n'' = (Main,nx'')` `\<forall>a\<in>set as. intra_kind (kind a)` `nx'' \<noteq> Entry`]
   have path:"wfp' \<turnstile> (Main, nx'' \<oplus> 1) -as \<oplus>s 1\<rightarrow>* (p', n' \<oplus> 1)" .
-  from `valid_edge wfp a` `sourcenode a = (Main, nx)` `targetnode a = n''`
-    `n'' = (Main,nx'')` `nx \<noteq> Entry` `intra_kind (kind a)` wf
-  have "if (b) prog else c\<^isub>2,procs \<turnstile> (Main, nx \<oplus> 1) -kind a\<rightarrow> (Main, nx'' \<oplus> 1)"
+  from `valid_edge wfp a` `sourcenode a = (Main, n)` `targetnode a = n''`
+    `n'' = (Main,nx'')` `n \<noteq> Entry` `intra_kind (kind a)` wf
+  have "if (b) prog else c\<^isub>2,procs \<turnstile> (Main, n \<oplus> 1) -kind a\<rightarrow> (Main, nx'' \<oplus> 1)"
     by(fastsimp intro:PCFG_Main_edge_CondTrue_source_not_Entry simp:valid_edge_def)
-  with path `sourcenode a = (Main, nx)` `targetnode a = n''`
-    `n'' = (Main,nx'')` show ?case
+  with path `sourcenode a = (Main, n)` `targetnode a = n''` `n'' = (Main,nx'')`
+  show ?case
     apply(cases a) apply(clarsimp simp:label_incrs_def)
     by(auto intro:ProcCFG.Cons_path simp:valid_edge_def)
 qed
@@ -727,7 +737,7 @@ proof -
       from `n \<noteq> Entry` `prog \<turnstile> nx -IEdge (kind a)\<rightarrow>\<^isub>p nx'`
       have "if (b) c\<^isub>1 else prog \<turnstile> n \<oplus> (#:c\<^isub>1 + 1) -IEdge (kind a)\<rightarrow>\<^isub>p nx' \<oplus> (#:c\<^isub>1 + 1)"
 	by(fastsimp intro:Proc_CFG_edge_CondFalse_source_not_Entry)
-      hence "if (b) c\<^isub>1 else prog,procs \<turnstile> (Main,n \<oplus> (#:c\<^isub>1 + 1)) -(kind a)\<rightarrow> 
+      hence "if (b) c\<^isub>1 else prog,procs \<turnstile> (Main,n \<oplus> (#:c\<^isub>1 + 1)) -kind a\<rightarrow> 
 	(Main,nx' \<oplus> (#:c\<^isub>1 + 1))" by(rule PCFG.Main)
       thus ?thesis by(simp add:ProcCFG.valid_node_def)(fastsimp simp:valid_edge_def)
     next
@@ -760,15 +770,18 @@ proof -
 	with `prog \<turnstile> nx -IEdge (kind a)\<rightarrow>\<^isub>p nx'`
 	have "if (b) c\<^isub>1 else prog \<turnstile> nx \<oplus> (#:c\<^isub>1 + 1) -IEdge (kind a)\<rightarrow>\<^isub>p nx' \<oplus> (#:c\<^isub>1 + 1)"
 	  by(fastsimp intro:Proc_CFG_edge_CondFalse_source_not_Entry)
-	hence "if (b) c\<^isub>1 else prog,procs \<turnstile> (Main,nx \<oplus> (#:c\<^isub>1 + 1)) 
-	  -(kind a)\<rightarrow> (Main,nx' \<oplus> (#:c\<^isub>1 + 1))" by(rule PCFG.Main)
+	hence "if (b) c\<^isub>1 else prog,procs \<turnstile> (Main,nx \<oplus> (#:c\<^isub>1 + 1)) -kind a\<rightarrow> 
+          (Main,nx' \<oplus> (#:c\<^isub>1 + 1))" by(rule PCFG.Main)
 	with `(Main, n) = targetnode a` `(Main, nx') = targetnode a`[THEN sym] 
 	show ?thesis by(simp add:ProcCFG.valid_node_def)(fastsimp simp:valid_edge_def)
       qed
     qed
   next
-    case (Proc p ins outs c nx n' ps es rets)
-    from Proc(4)[THEN sym] Proc(5)[THEN sym] Proc(1-3,6-8) have False by fastsimp
+    case (Proc p ins outs c nx n' ps)
+    from `(p, nx) = sourcenode a`[THEN sym] `(p, n') = targetnode a`[THEN sym]
+      `(p, ins, outs, c) \<in> set procs` `well_formed procs`
+      `(Main, n) = sourcenode a \<or> (Main, n) = targetnode a`
+    have False by fastsimp
     thus ?case by simp
   next
     case (MainCall l p es rets n' ins outs c)
@@ -779,15 +792,17 @@ proof -
     from `prog \<turnstile> Label l -CEdge (p, es, rets)\<rightarrow>\<^isub>p n'`
     have "if (b) c\<^isub>1 else prog \<turnstile> Label l \<oplus> (#:c\<^isub>1 + 1) -CEdge (p, es, rets)\<rightarrow>\<^isub>p 
       n' \<oplus> (#:c\<^isub>1 + 1)" by -(rule Proc_CFG_edge_CondFalse_source_not_Entry,auto)
-    with `(p, ins, outs, c) \<in> set procs` `distinct rets`
-      `length rets = length outs` `length es = length ins`
+    with `(p, ins, outs, c) \<in> set procs`
     have "if (b) c\<^isub>1 else prog,procs \<turnstile> (Main,Label (l + (#:c\<^isub>1 + 1))) 
       -(\<lambda>s. True):(Main,n' \<oplus> (#:c\<^isub>1 + 1))\<hookrightarrow>\<^bsub>p\<^esub>map (\<lambda>e cf. interpret e cf) es\<rightarrow> (p,Entry)"
       by(fastsimp intro:PCFG.MainCall)
     thus ?case by(simp add:ProcCFG.valid_node_def)(fastsimp simp:valid_edge_def)
   next
-    case (ProcCall i p ins outs c l p' es' rets' l' ins' outs' c' ps es rets)
-    from ProcCall(9)[THEN sym] ProcCall(11)[THEN sym] ProcCall(1-8,10,12-14)
+    case (ProcCall p ins outs c l p' es' rets' l' ins' outs' c' ps)
+    from `(p, Label l) = sourcenode a`[THEN sym]
+      `(p', Entry) = targetnode a`[THEN sym]  `well_formed procs`
+      `(p, ins, outs, c) \<in> set procs` `(p', ins', outs', c') \<in> set procs`
+      `(Main, n) = sourcenode a \<or> (Main, n) = targetnode a`
     have False by fastsimp
     thus ?case by simp
   next
@@ -799,16 +814,18 @@ proof -
     from `prog \<turnstile> Label l -CEdge (p, es, rets)\<rightarrow>\<^isub>p Label l'`
     have "if (b) c\<^isub>1 else prog \<turnstile> Label l \<oplus> (#:c\<^isub>1 + 1) -CEdge (p, es, rets)\<rightarrow>\<^isub>p 
       Label l' \<oplus> (#:c\<^isub>1 + 1)" by -(rule Proc_CFG_edge_CondFalse_source_not_Entry,auto)
-    with `(p, ins, outs, c) \<in> set procs` `distinct rets`
-      `length rets = length outs` `length es = length ins`
+    with `(p, ins, outs, c) \<in> set procs`
     have "if (b) c\<^isub>1 else prog,procs \<turnstile> (p,Exit) 
       -(\<lambda>cf. snd cf = (Main,Label l' \<oplus> (#:c\<^isub>1 + 1)))\<hookleftarrow>\<^bsub>p\<^esub>
       (\<lambda>cf cf'. cf'(rets [:=] map cf outs))\<rightarrow> (Main,Label (l' + (#:c\<^isub>1 + 1)))"
       by(fastsimp intro:PCFG.MainReturn)
     thus ?case by(simp add:ProcCFG.valid_node_def)(fastsimp simp:valid_edge_def)
   next
-    case (ProcReturn i p ins outs c l p' es' rets' l' ins' outs' c' ps es rets)
-    from ProcReturn(9)[THEN sym] ProcReturn(11)[THEN sym] ProcReturn(1-8,10,12-14)
+    case (ProcReturn p ins outs c l p' es' rets' l' ins' outs' c' ps)
+    from `(p', Exit) = sourcenode a`[THEN sym] 
+      `(p, Label l') = targetnode a`[THEN sym] `well_formed procs`
+      `(p, ins, outs, c) \<in> set procs` `(p', ins', outs', c') \<in> set procs`
+      `(Main, n) = sourcenode a \<or> (Main, n) = targetnode a`
     have False by fastsimp
     thus ?case by simp
   next
@@ -820,8 +837,7 @@ proof -
       from `n \<noteq> Entry` `prog \<turnstile> nx -CEdge (p, es, rets)\<rightarrow>\<^isub>p nx'`
       have "if (b) c\<^isub>1 else prog \<turnstile> n \<oplus> (#:c\<^isub>1 + 1) -CEdge (p, es, rets)\<rightarrow>\<^isub>p 
 	nx' \<oplus> (#:c\<^isub>1 + 1)" by(fastsimp intro:Proc_CFG_edge_CondFalse_source_not_Entry)
-      with `distinct rets`
-      have "if (b) c\<^isub>1 else prog,procs \<turnstile> (Main,n \<oplus> (#:c\<^isub>1 + 1)) 
+      hence "if (b) c\<^isub>1 else prog,procs \<turnstile> (Main,n \<oplus> (#:c\<^isub>1 + 1)) 
 	-(\<lambda>s. False)\<^isub>\<surd>\<rightarrow> (Main,nx' \<oplus> (#:c\<^isub>1 + 1))" by -(rule PCFG.MainCallReturn)
       thus ?thesis by(simp add:ProcCFG.valid_node_def)(fastsimp simp:valid_edge_def)
     next
@@ -831,16 +847,17 @@ proof -
       with `prog \<turnstile> nx -CEdge (p, es, rets)\<rightarrow>\<^isub>p nx'`
       have "if (b) c\<^isub>1 else prog \<turnstile> nx \<oplus> (#:c\<^isub>1 + 1) -CEdge (p, es, rets)\<rightarrow>\<^isub>p 
 	nx' \<oplus> (#:c\<^isub>1 + 1)" by(fastsimp intro:Proc_CFG_edge_CondFalse_source_not_Entry)
-      with `distinct rets`
-      have "if (b) c\<^isub>1 else prog,procs \<turnstile> (Main,nx \<oplus> (#:c\<^isub>1 + 1)) 
+      hence "if (b) c\<^isub>1 else prog,procs \<turnstile> (Main,nx \<oplus> (#:c\<^isub>1 + 1)) 
 	-(\<lambda>s. False)\<^isub>\<surd>\<rightarrow> (Main,nx' \<oplus> (#:c\<^isub>1 + 1))" by -(rule PCFG.MainCallReturn)
       with `(Main, n) = targetnode a` `(Main, nx') = targetnode a`[THEN sym]
       show ?thesis by(simp add:ProcCFG.valid_node_def)(fastsimp simp:valid_edge_def)
     qed
   next
-    case (ProcCallReturn p ins outs c nx p' es' rets' n' ps es rets)
-    from ProcCallReturn(5)[THEN sym] ProcCallReturn(7)[THEN sym]
-      ProcCallReturn(1-4,6,8-10) have False by fastsimp
+    case (ProcCallReturn p ins outs c nx p' es' rets' n' ps)
+    from `(p, nx) = sourcenode a`[THEN sym] `(p, n') = targetnode a`[THEN sym]
+      `(p, ins, outs, c) \<in> set procs` `well_formed procs`
+      `(Main, n) = sourcenode a \<or> (Main, n) = targetnode a`
+    have False by fastsimp
     thus ?case by simp
   qed
 qed
@@ -861,8 +878,8 @@ proof(induct "(Main,n)" as "(p',n')" arbitrary:n rule:ProcCFG.path.induct)
   with `Main = p'` show ?case
     by(fastsimp intro:ProcCFG.empty_path simp:label_incrs_def)
 next
-  case (Cons_path n'' as a nx)
-  note IH = `\<And>n.  \<lbrakk>n'' = (Main, n); \<forall>a\<in>set as. intra_kind (kind a); n \<noteq> Entry\<rbrakk>
+  case (Cons_path n'' as a n)
+  note IH = `\<And>n. \<And>n.  \<lbrakk>n'' = (Main, n); \<forall>a\<in>set as. intra_kind (kind a); n \<noteq> Entry\<rbrakk>
     \<Longrightarrow> wfp' \<turnstile> (Main, n \<oplus> (#:c\<^isub>1 + 1)) -as \<oplus>s (#:c\<^isub>1 + 1)\<rightarrow>* (p', n' \<oplus> (#:c\<^isub>1 + 1))`
   note [simp] = `Rep_wf_prog wfp = (prog,procs)` 
     `Rep_wf_prog wfp' = (if (b) c\<^isub>1 else prog,procs)`
@@ -870,20 +887,20 @@ next
     by(fastsimp intro:wf_wf_prog)
   from `\<forall>a\<in>set (a # as). intra_kind (kind a)` have "intra_kind (kind a)"
     and "\<forall>a\<in>set as. intra_kind (kind a)" by simp_all
-  from `valid_edge wfp a` `sourcenode a = (Main, nx)` `targetnode a = n''`
+  from `valid_edge wfp a` `sourcenode a = (Main, n)` `targetnode a = n''`
     `intra_kind (kind a)` wf 
   obtain nx'' where "n'' = (Main,nx'')" and "nx'' \<noteq> Entry"
     by(auto elim!:PCFG.cases simp:valid_edge_def intra_kind_def)
   from IH[OF `n'' = (Main,nx'')` `\<forall>a\<in>set as. intra_kind (kind a)` `nx'' \<noteq> Entry`]
-  have path:"wfp' \<turnstile> (Main, nx'' \<oplus> (#:c\<^isub>1 + 1)) 
-    -as \<oplus>s (#:c\<^isub>1 + 1)\<rightarrow>* (p', n' \<oplus> (#:c\<^isub>1 + 1))" .
-  from `valid_edge wfp a` `sourcenode a = (Main, nx)` `targetnode a = n''`
-    `n'' = (Main,nx'')` `nx \<noteq> Entry` `intra_kind (kind a)` wf
-  have "if (b) c\<^isub>1 else prog,procs \<turnstile> (Main, nx \<oplus> (#:c\<^isub>1 + 1)) -kind a\<rightarrow> 
+  have path:"wfp' \<turnstile> (Main, nx'' \<oplus> (#:c\<^isub>1 + 1)) -as \<oplus>s (#:c\<^isub>1 + 1)\<rightarrow>* 
+    (p', n' \<oplus> (#:c\<^isub>1 + 1))" .
+  from `valid_edge wfp a` `sourcenode a = (Main, n)` `targetnode a = n''`
+    `n'' = (Main,nx'')` `n \<noteq> Entry` `intra_kind (kind a)` wf
+  have "if (b) c\<^isub>1 else prog,procs \<turnstile> (Main, n \<oplus> (#:c\<^isub>1 + 1)) -kind a\<rightarrow> 
     (Main, nx'' \<oplus> (#:c\<^isub>1 + 1))"
     by(fastsimp intro:PCFG_Main_edge_CondFalse_source_not_Entry simp:valid_edge_def)
-  with path `sourcenode a = (Main, nx)` `targetnode a = n''`
-    `n'' = (Main,nx'')` show ?case
+  with path `sourcenode a = (Main, n)` `targetnode a = n''` `n'' = (Main,nx'')`
+  show ?case
     apply(cases a) apply(clarsimp simp:label_incrs_def)
     by(auto intro:ProcCFG.Cons_path simp:valid_edge_def)
 qed
@@ -940,7 +957,7 @@ proof -
 	with `n \<noteq> Entry` `prog \<turnstile> nx -IEdge (kind a)\<rightarrow>\<^isub>p nx'`
 	have "while (b) prog \<turnstile> n \<oplus> 2 -IEdge (kind a)\<rightarrow>\<^isub>p Label 0"
 	  by(fastsimp intro:Proc_CFG_WhileBodyExit)
-	hence "while (b) prog,procs \<turnstile> (Main,n \<oplus> 2) -(kind a)\<rightarrow> (Main,Label 0)"
+	hence "while (b) prog,procs \<turnstile> (Main,n \<oplus> 2) -kind a\<rightarrow> (Main,Label 0)"
 	  by(rule PCFG.Main)
 	thus ?thesis by(simp add:ProcCFG.valid_node_def)(fastsimp simp:valid_edge_def)
       next
@@ -948,7 +965,7 @@ proof -
 	with `n \<noteq> Entry` `prog \<turnstile> nx -IEdge (kind a)\<rightarrow>\<^isub>p nx'`
 	have "while (b) prog \<turnstile> n \<oplus> 2 -IEdge (kind a)\<rightarrow>\<^isub>p nx' \<oplus> 2"
 	  by(fastsimp intro:Proc_CFG_edge_WhileBody_source_not_Entry)
-	hence "while (b) prog,procs \<turnstile> (Main,n \<oplus> 2) -(kind a)\<rightarrow> (Main,nx' \<oplus> 2)"
+	hence "while (b) prog,procs \<turnstile> (Main,n \<oplus> 2) -kind a\<rightarrow> (Main,nx' \<oplus> 2)"
 	  by(rule PCFG.Main)
 	thus ?thesis by(simp add:ProcCFG.valid_node_def)(fastsimp simp:valid_edge_def)
       qed
@@ -988,8 +1005,8 @@ proof -
 	  with `prog \<turnstile> nx -IEdge (kind a)\<rightarrow>\<^isub>p nx'` `nx \<noteq> Entry`
 	  have "while (b) prog \<turnstile> nx \<oplus> 2 -IEdge (kind a)\<rightarrow>\<^isub>p nx' \<oplus> 2"
 	    by(fastsimp intro:Proc_CFG_edge_WhileBody_source_not_Entry)
-	  hence "while (b) prog,procs \<turnstile> (Main,nx \<oplus> 2) 
-	    -(kind a)\<rightarrow> (Main,nx' \<oplus> 2)" by(rule PCFG.Main)
+	  hence "while (b) prog,procs \<turnstile> (Main,nx \<oplus> 2)  -kind a\<rightarrow> 
+            (Main,nx' \<oplus> 2)" by(rule PCFG.Main)
 	  with `(Main, n) = targetnode a` `(Main, nx') = targetnode a`[THEN sym]
 	  show ?thesis
 	    by(simp add:ProcCFG.valid_node_def)(fastsimp simp:valid_edge_def)
@@ -997,8 +1014,11 @@ proof -
       qed
     qed
   next
-    case (Proc p ins outs c nx n' ps es rets)
-    from Proc(4)[THEN sym] Proc(5)[THEN sym] Proc(1-3,6-8) have False by fastsimp
+    case (Proc p ins outs c nx n' ps)
+    from `(p, nx) = sourcenode a`[THEN sym] `(p, n') = targetnode a`[THEN sym]
+      `(Main, n) = sourcenode a \<or> (Main, n) = targetnode a` 
+      `(p, ins, outs, c) \<in> set procs` `well_formed procs` 
+    have False by fastsimp
     thus ?case by simp
   next
     case (MainCall l p es rets n' ins outs c)
@@ -1011,15 +1031,17 @@ proof -
     with `prog \<turnstile> Label l -CEdge (p, es, rets)\<rightarrow>\<^isub>p n'`
     have "while (b) prog \<turnstile> Label l \<oplus> 2 -CEdge (p, es, rets)\<rightarrow>\<^isub>p 
       n' \<oplus> 2" by -(rule Proc_CFG_edge_WhileBody_source_not_Entry,auto)
-    with `(p, ins, outs, c) \<in> set procs` `distinct rets`
-      `length rets = length outs` `length es = length ins`
+    with `(p, ins, outs, c) \<in> set procs`
     have "while (b) prog,procs \<turnstile> (Main,Label l \<oplus> 2) 
       -(\<lambda>s. True):(Main,n' \<oplus> 2)\<hookrightarrow>\<^bsub>p\<^esub>map (\<lambda>e cf. interpret e cf) es\<rightarrow> (p,Entry)"
       by(fastsimp intro:PCFG.MainCall)
     thus ?case by(simp add:ProcCFG.valid_node_def)(fastsimp simp:valid_edge_def)
   next
-    case (ProcCall i p ins outs c l p' es' rets' l' ins' outs' c' ps es rets)
-    from ProcCall(9)[THEN sym] ProcCall(11)[THEN sym] ProcCall(1-8,10,12-14)
+    case (ProcCall p ins outs c l p' es' rets' l' ins' outs' c')
+    from `(p, Label l) = sourcenode a`[THEN sym]
+      `(p', Entry) = targetnode a`[THEN sym]  `well_formed procs`
+      `(p, ins, outs, c) \<in> set procs` `(p', ins', outs', c') \<in> set procs`
+      `(Main, n) = sourcenode a \<or> (Main, n) = targetnode a`
     have False by fastsimp
     thus ?case by simp
   next
@@ -1031,15 +1053,17 @@ proof -
     from `prog \<turnstile> Label l -CEdge (p, es, rets)\<rightarrow>\<^isub>p Label l'`
     have "while (b) prog \<turnstile> Label l \<oplus> 2 -CEdge (p, es, rets)\<rightarrow>\<^isub>p 
       Label l' \<oplus> 2" by -(rule Proc_CFG_edge_WhileBody_source_not_Entry,auto)
-    with `(p, ins, outs, c) \<in> set procs` `distinct rets`
-      `length rets = length outs` `length es = length ins`
+    with `(p, ins, outs, c) \<in> set procs`
     have "while (b) prog,procs \<turnstile> (p,Exit) -(\<lambda>cf. snd cf = (Main,Label l' \<oplus> 2))\<hookleftarrow>\<^bsub>p\<^esub>
       (\<lambda>cf cf'. cf'(rets [:=] map cf outs))\<rightarrow> (Main,Label l' \<oplus> 2)"
       by(fastsimp intro:PCFG.MainReturn)
     thus ?case by(simp add:ProcCFG.valid_node_def)(fastsimp simp:valid_edge_def)
   next
-    case (ProcReturn i p ins outs c l p' es' rets' l' ins' outs' c' ps es rets)
-    from ProcReturn(9)[THEN sym] ProcReturn(11)[THEN sym] ProcReturn(1-8,10,12-14)
+    case (ProcReturn p ins outs c l p' es' rets' l' ins' outs' c' ps)
+    from `(p', Exit) = sourcenode a`[THEN sym] 
+      `(p, Label l') = targetnode a`[THEN sym] `well_formed procs`
+      `(p, ins, outs, c) \<in> set procs` `(p', ins', outs', c') \<in> set procs`
+      `(Main, n) = sourcenode a \<or> (Main, n) = targetnode a`
     have False by fastsimp
     thus ?case by simp
   next
@@ -1053,8 +1077,7 @@ proof -
       with `n \<noteq> Entry` `prog \<turnstile> nx -CEdge (p, es, rets)\<rightarrow>\<^isub>p nx'`
       have "while (b) prog \<turnstile> n \<oplus> 2 -CEdge (p, es, rets)\<rightarrow>\<^isub>p 
 	nx' \<oplus> 2" by(fastsimp intro:Proc_CFG_edge_WhileBody_source_not_Entry)
-      with `distinct rets`
-      have "while (b) prog,procs \<turnstile> (Main,n \<oplus> 2) -(\<lambda>s. False)\<^isub>\<surd>\<rightarrow> (Main,nx' \<oplus> 2)"
+      hence "while (b) prog,procs \<turnstile> (Main,n \<oplus> 2) -(\<lambda>s. False)\<^isub>\<surd>\<rightarrow> (Main,nx' \<oplus> 2)"
 	by -(rule PCFG.MainCallReturn)
       thus ?thesis by(simp add:ProcCFG.valid_node_def)(fastsimp simp:valid_edge_def)
     next
@@ -1064,16 +1087,17 @@ proof -
       with `prog \<turnstile> nx -CEdge (p, es, rets)\<rightarrow>\<^isub>p nx'`
       have "while (b) prog \<turnstile> nx \<oplus> 2 -CEdge (p, es, rets)\<rightarrow>\<^isub>p 
 	nx' \<oplus> 2" by(fastsimp intro:Proc_CFG_edge_WhileBody_source_not_Entry)
-      with `distinct rets`
-      have "while (b) prog,procs \<turnstile> (Main,nx \<oplus> 2) -(\<lambda>s. False)\<^isub>\<surd>\<rightarrow> (Main,nx' \<oplus> 2)"
+      hence "while (b) prog,procs \<turnstile> (Main,nx \<oplus> 2) -(\<lambda>s. False)\<^isub>\<surd>\<rightarrow> (Main,nx' \<oplus> 2)"
 	by -(rule PCFG.MainCallReturn)
       with `(Main, n) = targetnode a` `(Main, nx') = targetnode a`[THEN sym] 
       show ?thesis by(simp add:ProcCFG.valid_node_def)(fastsimp simp:valid_edge_def)
     qed
   next
-    case (ProcCallReturn p ins outs c nx p' es' rets' n' ps es rets)
-    from ProcCallReturn(5)[THEN sym] ProcCallReturn(7)[THEN sym]
-      ProcCallReturn(1-4,6,8-10) have False by fastsimp
+    case (ProcCallReturn p ins outs c nx p' es' rets' n' ps)
+    from `(p, nx) = sourcenode a`[THEN sym] `(p, n') = targetnode a`[THEN sym]
+      `(p, ins, outs, c) \<in> set procs` `well_formed procs`
+      `(Main, n) = sourcenode a \<or> (Main, n) = targetnode a`
+    have False by fastsimp
     thus ?case by simp
   qed
 qed
@@ -1094,8 +1118,8 @@ proof(induct "(Main,n)" as "(p',n')" arbitrary:n rule:ProcCFG.path.induct)
   with `Main = p'` show ?case
     by(fastsimp intro:ProcCFG.empty_path simp:label_incrs_def)
 next
-  case (Cons_path n'' as a nx)
-  note IH = `\<And>n.  \<lbrakk>n'' = (Main, n); \<forall>a\<in>set as. intra_kind (kind a); n \<noteq> Entry;
+  case (Cons_path n'' as a n)
+  note IH = `\<And>n.  \<lbrakk>n'' = (Main, n); \<forall>a\<in>set as. intra_kind (kind a); n \<noteq> Entry; 
     n' \<noteq> Exit\<rbrakk> \<Longrightarrow> wfp' \<turnstile> (Main, n \<oplus> 2) -as \<oplus>s 2\<rightarrow>* (p', n' \<oplus> 2)`
   note [simp] = `Rep_wf_prog wfp = (prog,procs)` 
      `Rep_wf_prog wfp' = (while (b) prog,procs)`
@@ -1103,20 +1127,20 @@ next
     by(fastsimp intro:wf_wf_prog)
   from `\<forall>a\<in>set (a # as). intra_kind (kind a)` have "intra_kind (kind a)"
     and "\<forall>a\<in>set as. intra_kind (kind a)" by simp_all
-  from `valid_edge wfp a` `sourcenode a = (Main, nx)` `targetnode a = n''`
+  from `valid_edge wfp a` `sourcenode a = (Main, n)` `targetnode a = n''`
     `intra_kind (kind a)` wf 
   obtain nx'' where "n'' = (Main,nx'')" and "nx'' \<noteq> Entry"
     by(auto elim!:PCFG.cases simp:valid_edge_def intra_kind_def)
-  from IH[OF `n'' = (Main,nx'')` `\<forall>a\<in>set as. intra_kind (kind a)` `nx'' \<noteq> Entry`
-    `n' \<noteq> Exit`]
+  from IH[OF `n'' = (Main,nx'')` `\<forall>a\<in>set as. intra_kind (kind a)` 
+    `nx'' \<noteq> Entry` `n' \<noteq> Exit`]
   have path:"wfp' \<turnstile> (Main, nx'' \<oplus> 2) -as \<oplus>s 2\<rightarrow>* (p', n' \<oplus> 2)" .
   with `n' \<noteq> Exit` have "nx'' \<noteq> Exit" by(fastsimp dest:ProcCFGExit.path_Exit_source)
-  with `valid_edge wfp a` `sourcenode a = (Main, nx)` `targetnode a = n''`
-    `n'' = (Main,nx'')` `nx \<noteq> Entry` `intra_kind (kind a)` wf
-  have "while (b) prog,procs \<turnstile> (Main, nx \<oplus> 2) -kind a\<rightarrow> (Main, nx'' \<oplus> 2)"
+  with `valid_edge wfp a` `sourcenode a = (Main, n)` `targetnode a = n''`
+    `n'' = (Main,nx'')` `n \<noteq> Entry` `intra_kind (kind a)` wf
+  have "while (b) prog,procs \<turnstile> (Main, n \<oplus> 2) -kind a\<rightarrow> (Main, nx'' \<oplus> 2)"
     by(fastsimp intro:PCFG_Main_edge_WhileBody_source_not_Entry simp:valid_edge_def)
-  with path `sourcenode a = (Main, nx)` `targetnode a = n''`
-    `n'' = (Main,nx'')` show ?case
+  with path `sourcenode a = (Main, n)` `targetnode a = n''` `n'' = (Main,nx'')`
+  show ?case
     apply(cases a) apply(clarsimp simp:label_incrs_def)
     by(auto intro:ProcCFG.Cons_path simp:valid_edge_def)
 qed
@@ -1534,13 +1558,10 @@ proof(atomize_elim)
   next
     case (Call p es rets)
     note Rep [simp] = `Rep_wf_prog wfp = (Call p es rets, procs)`
-    have cC:"containsCall procs (Call p es rets) [] p es rets" by simp
-    have "distinct rets"
-      by(fastsimp intro:wf_distinct_rets[OF _ cC] wf_wf_prog[OF Rep])
+    have cC:"containsCall procs (Call p es rets) [] p" by simp
     show ?case
     proof(cases "l = 0")
       case True
-      from `distinct rets` 
       have "wfp \<turnstile> (Main,Label 0) -((Main,Label 0),(\<lambda>s. False)\<^isub>\<surd>,(Main,Label 1))#
 	[((Main,Label 1),\<Up>id,(Main,Exit))]\<rightarrow>* (Main,Exit)"
 	by(fastsimp intro:ProcCFG.path.intros Main Proc_CFG_CallSkip MainCallReturn
@@ -1560,7 +1581,6 @@ proof(atomize_elim)
 	by(fastsimp intro:ProcCFG.path.intros Main Proc_CFG_CallSkip
 	            simp:valid_edge_def)
       moreover
-      from `distinct rets` 
       have "Call p es rets,procs \<turnstile> (Main,Label 0) -(\<lambda>s. False)\<^isub>\<surd>\<rightarrow> (Main,Label 1)"
 	by(fastsimp intro:MainCallReturn Proc_CFG_Call)
       hence "wfp \<turnstile> (Main,Entry) -((Main,Entry),(\<lambda>s. True)\<^isub>\<surd>,(Main,Label 0))#
@@ -1573,13 +1593,14 @@ proof(atomize_elim)
 qed
 
 
+
 subsection {* Lifting from edges in procedure Main to arbitrary procedures *}
 
 lemma lift_edge_Main_Main:
   "\<lbrakk>c,procs \<turnstile> (Main, n) -et\<rightarrow> (Main, n'); (p,ins,outs,c) \<in> set procs;
-  containsCall procs prog ps p es rets; well_formed procs\<rbrakk> 
+  containsCall procs prog ps p; well_formed procs\<rbrakk> 
   \<Longrightarrow> prog,procs \<turnstile> (p, n) -et\<rightarrow> (p, n')"
-proof(induct x\<equiv>"(Main,n)" et x'\<equiv>"(Main,n')" rule:PCFG.induct)
+proof(induct "(Main,n)" et "(Main,n')" rule:PCFG.induct)
   case Main thus ?case by(fastsimp intro:Proc)
 next
   case MainCallReturn thus ?case by(fastsimp intro:ProcCallReturn)
@@ -1587,32 +1608,29 @@ qed auto
 
 lemma lift_edge_Main_Proc:
   "\<lbrakk>c,procs \<turnstile> (Main, n) -et\<rightarrow> (q, n'); q \<noteq> Main; (p,ins,outs,c) \<in> set procs;
-  containsCall procs prog ps p es rets; well_formed procs\<rbrakk> 
+  containsCall procs prog ps p; well_formed procs\<rbrakk> 
   \<Longrightarrow> \<exists>et'. prog,procs \<turnstile> (p, n) -et'\<rightarrow> (q, n')"
 proof(induct "(Main,n)" et "(q,n')" rule:PCFG.induct)
   case (MainCall l esx retsx n'x insx outsx cx)
   from `c \<turnstile> Label l -CEdge (q, esx, retsx)\<rightarrow>\<^isub>p n'x` 
   obtain l' where [simp]:"n'x = Label l'" by(fastsimp dest:Proc_CFG_Call_Labels)
-  from `(p, ins, outs, c) \<in> set procs` obtain i where "i < length procs"
-    and "procs!i = (p, ins, outs, c)" by(auto simp:set_conv_nth)
-  with MainCall have "prog,procs \<turnstile> (p, Label l) 
-    -(\<lambda>s. True):(p,n'x)\<hookrightarrow>\<^bsub>q\<^esub>map (\<lambda>e cf. interpret e cf) esx\<rightarrow> (q, Entry)"
-    by(fastsimp intro!:ProcCall)
-  with `Label l = n` `Entry = n'` show ?case by fastsimp
+  with MainCall have "prog,procs \<turnstile> (p, n) 
+    -(\<lambda>s. True):(p,n'x)\<hookrightarrow>\<^bsub>q\<^esub>map (\<lambda>e cf. interpret e cf) esx\<rightarrow> (q, n')"
+    by(fastsimp intro:ProcCall)
+  thus ?case by fastsimp
 qed auto
 
 lemma lift_edge_Proc_Main:
   "\<lbrakk>c,procs \<turnstile> (q, n) -et\<rightarrow> (Main, n'); q \<noteq> Main; (p,ins,outs,c) \<in> set procs;
-  containsCall procs prog ps p es rets; well_formed procs\<rbrakk> 
+  containsCall procs prog ps p; well_formed procs\<rbrakk> 
   \<Longrightarrow> \<exists>et'. prog,procs \<turnstile> (q, n) -et'\<rightarrow> (p, n')"
 proof(induct "(q,n)" et "(Main,n')" rule:PCFG.induct)
   case (MainReturn l esx retsx l' insx outsx cx)
-  from `(p, ins, outs, c) \<in> set procs` obtain i where "i < length procs"
-    and "procs!i = (p, ins, outs, c)" by(auto simp:set_conv_nth)
-  with MainReturn have "prog,procs \<turnstile> (q,Exit) -(\<lambda>cf. snd cf = (p,Label l'))\<hookleftarrow>\<^bsub>q\<^esub>
+  note [simp] = `Exit = n`[THEN sym] `Label l' = n'`[THEN sym]
+  from MainReturn have "prog,procs \<turnstile> (q,Exit) -(\<lambda>cf. snd cf = (p,Label l'))\<hookleftarrow>\<^bsub>q\<^esub>
     (\<lambda>cf cf'. cf'(retsx [:=] map cf outsx))\<rightarrow> (p,Label l')"
     by(fastsimp intro!:ProcReturn)
-  with `Exit = n` `Label l' = n'` show ?case by fastsimp
+  thus ?case by fastsimp
 qed auto
 
 
@@ -1625,7 +1643,7 @@ fun lift_path :: "edge list \<Rightarrow> pname \<Rightarrow> edge list"
 
 lemma lift_path_Proc: 
   assumes "Rep_wf_prog wfp' = (c,procs)" and "Rep_wf_prog wfp = (prog,procs)"
-  and "(p,ins,outs,c) \<in> set procs" and "containsCall procs prog ps p es rets"
+  and "(p,ins,outs,c) \<in> set procs" and "containsCall procs prog ps p"
   shows "\<lbrakk>wfp' \<turnstile> (Main,n) -as\<rightarrow>* (Main,n'); \<forall>a \<in> set as. intra_kind (kind a)\<rbrakk>
   \<Longrightarrow> wfp \<turnstile> (p,n) -lift_path as p\<rightarrow>* (p,n')"
 proof(induct "(Main,n)" as "(Main,n')" arbitrary:n rule:ProcCFG.path.induct)
@@ -1651,13 +1669,13 @@ next
     by(fastsimp intro:wf_wf_prog)
   from `\<forall>a\<in>set (a # as). intra_kind (kind a)` have "intra_kind (kind a)"
     and "\<forall>a\<in>set as. intra_kind (kind a)" by simp_all
-  from `valid_edge wfp' a` `intra_kind (kind a)` `sourcenode a = (Main, n)`
+  from `valid_edge wfp' a` `intra_kind (kind a)` `sourcenode a = (Main, n)` 
     `targetnode a = m''` `Rep_wf_prog wfp' = (c,procs)`
   obtain n'' where "m'' = (Main, n'')"
     by(fastsimp elim:PCFG.cases simp:valid_edge_def intra_kind_def)
   with `valid_edge wfp' a` `Rep_wf_prog wfp' = (c,procs)`
     `sourcenode a = (Main, n)` `targetnode a = m''`
-    `(p,ins,outs,c) \<in> set procs` `containsCall procs prog ps p es rets` 
+    `(p,ins,outs,c) \<in> set procs` `containsCall procs prog ps p` 
     `Rep_wf_prog wfp = (prog,procs)` wf
   have "prog,procs \<turnstile> (p, n) -kind a\<rightarrow> (p, n'')"
     by(auto intro:lift_edge_Main_Main simp:valid_edge_def)  
@@ -1673,14 +1691,14 @@ subsection {* Existence of paths from Entry and to Exit *}
 
 lemma Label_Proc_CFG_Entry_Exit_path_Proc:
   assumes "Rep_wf_prog wfp = (prog,procs)" and "l < #:c"
-  and "(p,ins,outs,c) \<in> set procs" and "containsCall procs prog ps p es rets"
+  and "(p,ins,outs,c) \<in> set procs" and "containsCall procs prog ps p"
   obtains as as' where "wfp \<turnstile> (p,Label l) -as\<rightarrow>* (p,Exit)"
   and "\<forall>a \<in> set as. intra_kind (kind a)"
   and "wfp \<turnstile> (p,Entry) -as'\<rightarrow>* (p,Label l)"
   and "\<forall>a \<in> set as'. intra_kind (kind a)"
 proof(atomize_elim)
   from `Rep_wf_prog wfp = (prog,procs)` `(p,ins,outs,c) \<in> set procs`
-    `containsCall procs prog ps p es rets`
+    `containsCall procs prog ps p`
   obtain wfp' where "Rep_wf_prog wfp' = (c,procs)" by(erule wfp_Call)
   from this `l < #:c` obtain as as' where "wfp' \<turnstile> (Main,Label l) -as\<rightarrow>* (Main,Exit)"
     and "\<forall>a \<in> set as. intra_kind (kind a)"
@@ -1688,13 +1706,13 @@ proof(atomize_elim)
     and "\<forall>a \<in> set as'. intra_kind (kind a)" 
     by(erule Label_Proc_CFG_Entry_Exit_path_Main)
   from `Rep_wf_prog wfp' = (c,procs)` `Rep_wf_prog wfp = (prog,procs)`
-    `(p,ins,outs,c) \<in> set procs` `containsCall procs prog ps p es rets`
+    `(p,ins,outs,c) \<in> set procs` `containsCall procs prog ps p`
     `wfp' \<turnstile> (Main,Label l) -as\<rightarrow>* (Main,Exit)` `\<forall>a \<in> set as. intra_kind (kind a)`
   have "wfp \<turnstile> (p,Label l) -lift_path as p\<rightarrow>* (p,Exit)"
     by(fastsimp intro:lift_path_Proc)
   moreover
   from `Rep_wf_prog wfp' = (c,procs)` `Rep_wf_prog wfp = (prog,procs)`
-    `(p,ins,outs,c) \<in> set procs` `containsCall procs prog ps p es rets`
+    `(p,ins,outs,c) \<in> set procs` `containsCall procs prog ps p`
     `wfp' \<turnstile> (Main,Entry) -as'\<rightarrow>* (Main,Label l)` `\<forall>a \<in> set as'. intra_kind (kind a)`
   have "wfp \<turnstile> (p,Entry) -lift_path as' p\<rightarrow>* (p,Label l)"
     by(fastsimp intro:lift_path_Proc)
@@ -1711,36 +1729,27 @@ qed
 
 lemma Entry_to_Entry_and_Exit_to_Exit: 
   assumes "Rep_wf_prog wfp = (prog,procs)"
-  and "containsCall procs prog ps p es rets" and "(p,ins,outs,c) \<in> set procs"
+  and "containsCall procs prog ps p" and "(p,ins,outs,c) \<in> set procs"
   obtains as as' where "CFG.valid_path' sourcenode targetnode kind
       (valid_edge wfp) (get_return_edges wfp) (Main,Entry) as (p,Entry)"
   and "CFG.valid_path' sourcenode targetnode kind
       (valid_edge wfp) (get_return_edges wfp) (p,Exit) as' (Main,Exit)"
 proof(atomize_elim)
-  from `containsCall procs prog ps p es rets` `(p,ins,outs,c) \<in> set procs`
+  from `containsCall procs prog ps p` `(p,ins,outs,c) \<in> set procs`
   show "\<exists>as as'. CFG.valid_path' sourcenode targetnode kind (valid_edge wfp)
     (get_return_edges wfp) (Main, Entry) as (p, Entry) \<and>
     CFG.valid_path' sourcenode targetnode kind (valid_edge wfp)
     (get_return_edges wfp) (p, Exit) as' (Main, Exit)"
-  proof(induct ps arbitrary:p es rets ins outs c rule:rev_induct)
+  proof(induct ps arbitrary:p ins outs c rule:rev_induct)
     case Nil
-    from `containsCall procs prog [] p es rets`
-    obtain lx lx' where "prog \<turnstile> Label lx -CEdge (p,es,rets)\<rightarrow>\<^isub>p Label lx'"
+    from `containsCall procs prog [] p`
+    obtain lx es rets lx' where "prog \<turnstile> Label lx -CEdge (p,es,rets)\<rightarrow>\<^isub>p Label lx'"
       by(erule containsCall_empty_Proc_CFG_Call_edge)
-    moreover
-    from `Rep_wf_prog wfp = (prog,procs)` `containsCall procs prog [] p es rets`
-    have "distinct rets" by(fastsimp intro:wf_wf_prog)
-    moreover
-    from `Rep_wf_prog wfp = (prog,procs)` `containsCall procs prog [] p es rets`
-      `(p, ins, outs, c) \<in> set procs`
-    have "length rets = length outs" and "length es = length ins"
-      by(auto intro:wf_length_retsI wf_length_esI wf_wf_prog simp del:add_2_eq_Suc')
-    ultimately
+    with `(p, ins, outs, c) \<in> set procs`
     have "prog,procs \<turnstile> (Main,Label lx) -(\<lambda>s. True):(Main,Label lx')\<hookrightarrow>\<^bsub>p\<^esub>
       map (\<lambda>e cf. interpret e cf) es\<rightarrow>  (p,Entry)" 
       and "prog,procs \<turnstile> (p,Exit) -(\<lambda>cf. snd cf = (Main,Label lx'))\<hookleftarrow>\<^bsub>p\<^esub>
       (\<lambda>cf cf'. cf'(rets [:=] map cf outs))\<rightarrow> (Main,Label lx')"
-      using `(p, ins, outs, c) \<in> set procs`
       by -(rule MainCall,assumption+,rule MainReturn)
     with `Rep_wf_prog wfp = (prog,procs)`
     have "wfp \<turnstile> (Main,Label lx) -[((Main,Label lx),
@@ -1781,30 +1790,29 @@ proof(atomize_elim)
     ultimately show ?case by(fastsimp intro:ProcCFG.path_Append simp:ProcCFG.vp_def)
   next
     case (snoc p' ps')
-    note IH = `\<And>p es rets ins outs c. 
-      \<lbrakk>containsCall procs prog ps' p es rets; (p,ins,outs,c) \<in> set procs\<rbrakk>
+    note IH = `\<And>p ins outs c. 
+      \<lbrakk>containsCall procs prog ps' p; (p,ins,outs,c) \<in> set procs\<rbrakk>
       \<Longrightarrow> \<exists>as as'. CFG.valid_path' sourcenode targetnode kind (valid_edge wfp)
       (get_return_edges wfp) (Main, Entry) as (p, Entry) \<and>
       CFG.valid_path' sourcenode targetnode kind (valid_edge wfp)
       (get_return_edges wfp) (p, Exit) as' (Main, Exit)`
-    from `containsCall procs prog (ps' @ [p']) p es rets`
-    obtain ins' outs' c' es' rets' where "(p',ins',outs',c') \<in> set procs"
-      and "containsCall procs c' [] p es rets" 
-      and "containsCall procs prog ps' p' es' rets'" by(auto elim:containsCallE)
-    from IH[OF `containsCall procs prog ps' p' es' rets'` 
-      `(p',ins',outs',c') \<in> set procs`] 
+    from `containsCall procs prog (ps' @ [p']) p`
+    obtain ins' outs' c' where "(p',ins',outs',c') \<in> set procs"
+      and "containsCall procs c' [] p" 
+      and "containsCall procs prog ps' p'" by(auto elim:containsCallE)
+    from IH[OF `containsCall procs prog ps' p'` `(p',ins',outs',c') \<in> set procs`] 
     obtain as as' where pathE:"CFG.valid_path' sourcenode targetnode kind 
       (valid_edge wfp) (get_return_edges wfp) (Main, Entry) as (p', Entry)"
       and pathX:"CFG.valid_path' sourcenode targetnode kind (valid_edge wfp)
       (get_return_edges wfp) (p', Exit) as' (Main, Exit)" by blast
-    from `containsCall procs c' [] p es rets`
-    obtain lx lx' where edge:"c' \<turnstile> Label lx -CEdge (p,es,rets)\<rightarrow>\<^isub>p Label lx'"
+    from `containsCall procs c' [] p`
+    obtain lx es rets lx' where edge:"c' \<turnstile> Label lx -CEdge (p,es,rets)\<rightarrow>\<^isub>p Label lx'"
       by(erule containsCall_empty_Proc_CFG_Call_edge)
     hence "lx < #:c'" and "lx' < #:c'"
       by(auto intro:Proc_CFG_sourcelabel_less_num_nodes 
 	            Proc_CFG_targetlabel_less_num_nodes)
     from `lx < #:c'` `Rep_wf_prog wfp = (prog,procs)` `(p',ins',outs',c') \<in> set procs`
-      `containsCall procs prog ps' p' es' rets'` obtain asx 
+      `containsCall procs prog ps' p'` obtain asx 
       where "wfp \<turnstile> (p',Entry) -asx\<rightarrow>* (p',Label lx)"
       and "\<forall>a \<in> set asx. intra_kind (kind a)"
       by(fastsimp elim:Label_Proc_CFG_Entry_Exit_path_Proc)
@@ -1813,7 +1821,7 @@ proof(atomize_elim)
       by(fastsimp intro:ProcCFG.path_Append ProcCFG.valid_path_same_level_path_Append
 	ProcCFG.intras_same_level_path simp:ProcCFG.vp_def)
     from `lx' < #:c'` `Rep_wf_prog wfp = (prog,procs)`
-      `(p',ins',outs',c') \<in> set procs` `containsCall procs prog ps' p' es' rets'` 
+      `(p',ins',outs',c') \<in> set procs` `containsCall procs prog ps' p'` 
     obtain asx' where "wfp \<turnstile> (p',Label lx') -asx'\<rightarrow>* (p',Exit)"
       and "\<forall>a \<in> set asx'. intra_kind (kind a)"
       by(fastsimp elim:Label_Proc_CFG_Entry_Exit_path_Proc)
@@ -1821,26 +1829,12 @@ proof(atomize_elim)
       (valid_edge wfp) (get_return_edges wfp) (p', Label lx') (asx'@as') (Main, Exit)"
       by(fastsimp intro:ProcCFG.path_Append ProcCFG.same_level_path_valid_path_Append
 	ProcCFG.intras_same_level_path simp:ProcCFG.vp_def)
-    from `(p',ins',outs',c') \<in> set procs` obtain i where "i < length procs" 
-      and "procs!i = (p',ins',outs',c')" by(auto simp:set_conv_nth)
-    moreover
-    from `Rep_wf_prog wfp = (prog,procs)` `(p',ins',outs',c') \<in> set procs`
-      `containsCall procs prog ps' p' es' rets'`
-    obtain wfp' where "Rep_wf_prog wfp' = (c',procs)" by(erule wfp_Call)
-    with `containsCall procs c' [] p es rets`
-    have "distinct rets" by(fastsimp intro:wf_wf_prog)
-    moreover
-    from `Rep_wf_prog wfp' = (c',procs)` `containsCall procs c' [] p es rets`
-      `(p,ins,outs,c) \<in> set procs`
-    have "length rets = length outs" and "length es = length ins"
-      by(auto intro:wf_length_retsI wf_length_esI wf_wf_prog simp del:add_2_eq_Suc')
-    ultimately
+    from edge `(p,ins,outs,c) \<in> set procs` `(p',ins',outs',c') \<in> set procs`
+      `containsCall procs prog ps' p'`
     have "prog,procs \<turnstile> (p',Label lx) -(\<lambda>s. True):(p',Label lx')\<hookrightarrow>\<^bsub>p\<^esub>
       map (\<lambda>e cf. interpret e cf) es\<rightarrow> (p,Entry)"
       and "prog,procs \<turnstile> (p,Exit) -(\<lambda>cf. snd cf = (p',Label lx'))\<hookleftarrow>\<^bsub>p\<^esub>
       (\<lambda>cf cf'. cf'(rets [:=] map cf outs))\<rightarrow> (p',Label lx')"
-      using edge `(p,ins,outs,c) \<in> set procs`
-	`containsCall procs prog ps' p' es' rets'`
       by(fastsimp intro:ProcCall ProcReturn)+
     with `Rep_wf_prog wfp = (prog,procs)`
     have path:"wfp \<turnstile> (p',Label lx) -[((p',Label lx),(\<lambda>s. True):(p',Label lx')\<hookrightarrow>\<^bsub>p\<^esub>
@@ -1885,7 +1879,8 @@ proof -
   show ?thesis
   proof(induct "sourcenode a" "kind a" "targetnode a" rule:PCFG.induct)
     case (Main nx nx')
-    from disj Main(2)[THEN sym] Main(3)[THEN sym] have [simp]:"p = Main" by auto
+    from `(Main, nx) = sourcenode a`[THEN sym] `(Main, nx') = targetnode a`[THEN sym]
+      disj have [simp]:"p = Main" by auto
     have "prog,procs \<turnstile> (Main, Entry) -(\<lambda>s. False)\<^isub>\<surd>\<rightarrow> (Main, Exit)"
       by(fastsimp intro:PCFG.Main Proc_CFG_Entry_Exit)
     hence EXpath:"wfp \<turnstile> (Main,Entry) -[((Main,Entry),(\<lambda>s. False)\<^isub>\<surd>,(Main,Exit))]\<rightarrow>*
@@ -1895,7 +1890,8 @@ proof -
     show ?case
     proof(cases n)
       case (Label l)
-      with `prog \<turnstile> nx -IEdge (kind a)\<rightarrow>\<^isub>p nx'` disj Main(2)[THEN sym] Main(3)[THEN sym]
+      with `prog \<turnstile> nx -IEdge (kind a)\<rightarrow>\<^isub>p nx'` `(Main, nx) = sourcenode a`[THEN sym]
+        `(Main, nx') = targetnode a`[THEN sym] disj
       have "l < #:prog" by(auto intro:Proc_CFG_sourcelabel_less_num_nodes
 	Proc_CFG_targetlabel_less_num_nodes)
       with `Rep_wf_prog wfp = (prog,procs)` 
@@ -1921,17 +1917,18 @@ proof -
 	  simp:ProcCFG.intra_path_def intra_kind_def)
     qed
   next
-    case (Proc px ins outs c nx nx' ps es rets)
+    case (Proc px ins outs c nx nx' ps)
     from `(px, ins, outs, c) \<in> set procs` wf have [simp]:"px \<noteq> Main" by auto
-    from disj Proc(4)[THEN sym] Proc(5)[THEN sym] have [simp]:"p = px" by auto
+    from disj `(px, nx) = sourcenode a`[THEN sym] `(px, nx') = targetnode a`[THEN sym]
+    have [simp]:"p = px" by auto
     from `Rep_wf_prog wfp = (prog,procs)` 
-      `containsCall procs prog ps px es rets` `(px, ins, outs, c) \<in> set procs`
+      `containsCall procs prog ps px` `(px, ins, outs, c) \<in> set procs`
     obtain asx asx' where path:"CFG.valid_path' sourcenode targetnode kind
       (valid_edge wfp) (get_return_edges wfp) (Main,Entry) asx (px,Entry)"
       and path':"CFG.valid_path' sourcenode targetnode kind
       (valid_edge wfp) (get_return_edges wfp) (px,Exit) asx' (Main,Exit)"
       by -(erule Entry_to_Entry_and_Exit_to_Exit)+
-    from `containsCall procs prog ps px es rets` `(px, ins, outs, c) \<in> set procs`
+    from `containsCall procs prog ps px` `(px, ins, outs, c) \<in> set procs`
     have "prog,procs \<turnstile> (px, Entry) -(\<lambda>s. False)\<^isub>\<surd>\<rightarrow> (px, Exit)"
       by(fastsimp intro:PCFG.Proc Proc_CFG_Entry_Exit)
     hence EXpath:"wfp \<turnstile> (px,Entry) -[((px,Entry),(\<lambda>s. False)\<^isub>\<surd>,(px,Exit))]\<rightarrow>* 
@@ -1940,11 +1937,12 @@ proof -
     show ?case
     proof(cases n)
       case (Label l)
-      with `c \<turnstile> nx -IEdge (kind a)\<rightarrow>\<^isub>p nx'` disj Proc(4)[THEN sym] Proc(5)[THEN sym]
+      with `c \<turnstile> nx -IEdge (kind a)\<rightarrow>\<^isub>p nx'` disj `(px, nx) = sourcenode a`[THEN sym]
+        `(px, nx') = targetnode a`[THEN sym]
       have "l < #:c" by(auto intro:Proc_CFG_sourcelabel_less_num_nodes
 	Proc_CFG_targetlabel_less_num_nodes)
       with `Rep_wf_prog wfp = (prog,procs)` `(px, ins, outs, c) \<in> set procs` 
-	`containsCall procs prog ps px es rets`
+	`containsCall procs prog ps px`
       obtain as as' where "wfp \<turnstile> (px,Entry) -as\<rightarrow>* (px,Label l)"
 	and "\<forall>a \<in> set as. intra_kind (kind a)"
 	and "wfp \<turnstile> (px,Label l) -as'\<rightarrow>* (px,Exit)"
@@ -1979,7 +1977,8 @@ proof -
     from disj show ?case
     proof
       assume "(p,n) = sourcenode a"
-      with MainCall(6)[THEN sym] have [simp]:"n = Label l" "p = Main" by simp_all
+      with `(Main, Label l) = sourcenode a`[THEN sym] 
+      have [simp]:"n = Label l" "p = Main" by simp_all
       with `prog \<turnstile> Label l -CEdge (px, es, rets)\<rightarrow>\<^isub>p nx'` have "l < #:prog"
 	by(fastsimp intro:Proc_CFG_sourcelabel_less_num_nodes)
       with `Rep_wf_prog wfp = (prog,procs)` 
@@ -1992,15 +1991,16 @@ proof -
 	by(fastsimp intro:ProcCFG.intra_path_vp simp:ProcCFG.intra_path_def)
     next
       assume "(p,n) = targetnode a"
-      with MainCall(8)[THEN sym] have [simp]:"n = Entry" "p = px" by simp_all
+      with `(px, Entry) = targetnode a`[THEN sym] 
+      have [simp]:"n = Entry" "p = px" by simp_all
       from `prog \<turnstile> Label l -CEdge (px, es, rets)\<rightarrow>\<^isub>p nx'`
-      have "containsCall procs prog [] px es rets" 
+      have "containsCall procs prog [] px" 
 	by(rule Proc_CFG_Call_containsCall)
       with `Rep_wf_prog wfp = (prog,procs)` `(px, ins, outs, c) \<in> set procs`
       obtain as' where Xpath:"CFG.valid_path' sourcenode targetnode kind
 	(valid_edge wfp) (get_return_edges wfp) (px,Exit) as' (Main,Exit)"
 	by -(erule Entry_to_Entry_and_Exit_to_Exit)      
-      from `containsCall procs prog [] px es rets` `(px, ins, outs, c) \<in> set procs`
+      from `containsCall procs prog [] px` `(px, ins, outs, c) \<in> set procs`
       have "prog,procs \<turnstile> (px, Entry) -(\<lambda>s. False)\<^isub>\<surd>\<rightarrow> (px, Exit)"
 	by(fastsimp intro:PCFG.Proc Proc_CFG_Entry_Exit)
       hence "wfp \<turnstile> (px,Entry) -[((px,Entry),(\<lambda>s. False)\<^isub>\<surd>,(px,Exit))]\<rightarrow>* (px,Exit)"
@@ -2013,29 +2013,28 @@ proof -
 	by(fastsimp intro:ProcCFG.path_Append 
 	  ProcCFG.same_level_path_valid_path_Append ProcCFG.intras_same_level_path
 	  simp:intra_kind_def)+
-      with `containsCall procs prog [] px es rets` `Rep_wf_prog wfp = (prog,procs)`
+      with `containsCall procs prog [] px` `Rep_wf_prog wfp = (prog,procs)`
 	`(px, ins, outs, c) \<in> set procs`
       show ?thesis by(fastsimp elim:Entry_to_Entry_and_Exit_to_Exit)
     qed
   next
-    case (ProcCall i px ins outs c l p' es' rets' l' ins' outs' c' ps es rets)
-    from `i < length procs` `procs ! i = (px, ins, outs, c)`[THEN sym]
-    have "(px, ins, outs, c) \<in> set procs" by(auto simp:set_conv_nth)
+    case (ProcCall px ins outs c l p' es' rets' l' ins' outs' c' ps)
     from disj show ?case
     proof
       assume "(p,n) = sourcenode a"
-      with ProcCall(9)[THEN sym] have [simp]:"n = Label l" "p = px" by simp_all
+      with `(px, Label l) = sourcenode a`[THEN sym] 
+      have [simp]:"n = Label l" "p = px" by simp_all
       with `c \<turnstile> Label l -CEdge (p', es', rets')\<rightarrow>\<^isub>p Label l'` have "l < #:c"
 	by(fastsimp intro:Proc_CFG_sourcelabel_less_num_nodes)
       from `Rep_wf_prog wfp = (prog,procs)` `l < #:c` 
-	`containsCall procs prog ps px es rets` `(px, ins, outs, c) \<in> set procs`
+	`containsCall procs prog ps px` `(px, ins, outs, c) \<in> set procs`
       obtain as as' where "wfp \<turnstile> (px,Label l) -as\<rightarrow>* (px,Exit)"
 	and "\<forall>a \<in> set as. intra_kind (kind a)"
 	and "wfp \<turnstile> (px,Entry) -as'\<rightarrow>* (px,Label l)"
 	and "\<forall>a \<in> set as'. intra_kind (kind a)"
 	by -(erule Label_Proc_CFG_Entry_Exit_path_Proc)+
       moreover
-      from `Rep_wf_prog wfp = (prog,procs)` `containsCall procs prog ps px es rets`
+      from `Rep_wf_prog wfp = (prog,procs)` `containsCall procs prog ps px`
 	`(px, ins, outs, c) \<in> set procs` obtain asx asx' 
 	where" CFG.valid_path' sourcenode targetnode kind
 	(valid_edge wfp) (get_return_edges wfp) (Main,Entry) asx (px,Entry)"
@@ -2049,11 +2048,12 @@ proof -
 	  simp:ProcCFG.vp_def)
     next
       assume "(p,n) = targetnode a"
-      with ProcCall(11)[THEN sym] have [simp]:"n = Entry" "p = p'" by simp_all
+      with `(p', Entry) = targetnode a`[THEN sym] 
+      have [simp]:"n = Entry" "p = p'" by simp_all
       from `c \<turnstile> Label l -CEdge (p', es', rets')\<rightarrow>\<^isub>p Label l'`
-      have "containsCall procs c [] p' es' rets'" by(rule Proc_CFG_Call_containsCall)
-      with `containsCall procs prog ps px es rets` `(px, ins, outs, c) \<in> set procs`
-      have "containsCall procs prog (ps@[px]) p' es' rets'"
+      have "containsCall procs c [] p'" by(rule Proc_CFG_Call_containsCall)
+      with `containsCall procs prog ps px` `(px, ins, outs, c) \<in> set procs`
+      have "containsCall procs prog (ps@[px]) p'"
 	by(rule containsCall_in_proc)
       with `(p', ins', outs', c') \<in> set procs`
       have "prog,procs \<turnstile> (p', Entry) -(\<lambda>s. False)\<^isub>\<surd>\<rightarrow> (p', Exit)"
@@ -2063,7 +2063,7 @@ proof -
 	  simp:valid_edge_def ProcCFG.valid_node_def)
       moreover
       from `Rep_wf_prog wfp = (prog,procs)` `(p', ins', outs', c') \<in> set procs`
-	`containsCall procs prog (ps@[px]) p' es' rets'`
+	`containsCall procs prog (ps@[px]) p'`
       obtain as as' where "CFG.valid_path' sourcenode targetnode kind
 	(valid_edge wfp) (get_return_edges wfp) (Main,Entry) as (p',Entry)"
 	and "CFG.valid_path' sourcenode targetnode kind
@@ -2082,9 +2082,10 @@ proof -
     from disj show ?case
     proof
       assume "(p,n) = sourcenode a"
-      with MainReturn(6)[THEN sym] have [simp]:"n = Exit" "p = px" by simp_all
+      with `(px, Exit) = sourcenode a`[THEN sym] 
+      have [simp]:"n = Exit" "p = px" by simp_all
       from `prog \<turnstile> Label l -CEdge (px, es, rets)\<rightarrow>\<^isub>p Label l'`
-      have "containsCall procs prog [] px es rets" by(rule Proc_CFG_Call_containsCall)
+      have "containsCall procs prog [] px" by(rule Proc_CFG_Call_containsCall)
       with `(px, ins, outs, c) \<in> set procs`
       have "prog,procs \<turnstile> (px, Entry) -(\<lambda>s. False)\<^isub>\<surd>\<rightarrow> (px, Exit)"
 	by(fastsimp intro:PCFG.Proc Proc_CFG_Entry_Exit)
@@ -2093,7 +2094,7 @@ proof -
 	  simp:valid_edge_def ProcCFG.valid_node_def)
       moreover
       from `Rep_wf_prog wfp = (prog,procs)` `(px, ins, outs, c) \<in> set procs`
-	`containsCall procs prog [] px es rets`
+	`containsCall procs prog [] px`
       obtain as as' where "CFG.valid_path' sourcenode targetnode kind
 	(valid_edge wfp) (get_return_edges wfp) (Main,Entry) as (px,Entry)"
 	and "CFG.valid_path' sourcenode targetnode kind
@@ -2108,7 +2109,8 @@ proof -
 	  simp:intra_kind_def)+
     next
       assume "(p, n) = targetnode a"
-      with MainReturn(8)[THEN sym] have [simp]:"n = Label l'" "p = Main" by simp_all
+      with `(Main, Label l') = targetnode a`[THEN sym] 
+      have [simp]:"n = Label l'" "p = Main" by simp_all
       with `prog \<turnstile> Label l -CEdge (px, es, rets)\<rightarrow>\<^isub>p Label l'` have "l' < #:prog"
 	by(fastsimp intro:Proc_CFG_targetlabel_less_num_nodes)
       with `Rep_wf_prog wfp = (prog,procs)` 
@@ -2121,17 +2123,16 @@ proof -
 	by(fastsimp intro:ProcCFG.intra_path_vp simp:ProcCFG.intra_path_def)
     qed
   next
-    case (ProcReturn i px ins outs c l p' es' rets' l' ins' outs' c' ps es rets)
-    from `i < length procs` `procs ! i = (px, ins, outs, c)`[THEN sym]
-    have "(px, ins, outs, c) \<in> set procs" by(auto simp:set_conv_nth)
+    case (ProcReturn px ins outs c l p' es' rets' l' ins' outs' c' ps)
     from disj show ?case
     proof
       assume "(p,n) = sourcenode a"
-      with ProcReturn(9)[THEN sym] have [simp]:"n = Exit" "p = p'" by simp_all
+      with `(p', Exit) = sourcenode a`[THEN sym] 
+      have [simp]:"n = Exit" "p = p'" by simp_all
       from `c \<turnstile> Label l -CEdge (p', es', rets')\<rightarrow>\<^isub>p Label l'`
-      have "containsCall procs c [] p' es' rets'" by(rule Proc_CFG_Call_containsCall)
-      with `containsCall procs prog ps px es rets` `(px, ins, outs, c) \<in> set procs`
-      have "containsCall procs prog (ps@[px]) p' es' rets'"
+      have "containsCall procs c [] p'" by(rule Proc_CFG_Call_containsCall)
+      with `containsCall procs prog ps px` `(px, ins, outs, c) \<in> set procs`
+      have "containsCall procs prog (ps@[px]) p'"
 	by(rule containsCall_in_proc)
       with `(p', ins', outs', c') \<in> set procs`
       have "prog,procs \<turnstile> (p', Entry) -(\<lambda>s. False)\<^isub>\<surd>\<rightarrow> (p', Exit)"
@@ -2141,7 +2142,7 @@ proof -
 	  simp:valid_edge_def ProcCFG.valid_node_def)
       moreover
       from `Rep_wf_prog wfp = (prog,procs)` `(p', ins', outs', c') \<in> set procs`
-	`containsCall procs prog (ps@[px]) p' es' rets'`
+	`containsCall procs prog (ps@[px]) p'`
       obtain as as' where "CFG.valid_path' sourcenode targetnode kind
 	(valid_edge wfp) (get_return_edges wfp) (Main,Entry) as (p',Entry)"
 	and "CFG.valid_path' sourcenode targetnode kind
@@ -2156,18 +2157,19 @@ proof -
 	  simp:intra_kind_def)+
     next
       assume "(p, n) = targetnode a"
-      with ProcReturn(11)[THEN sym] have [simp]:"n = Label l'" "p = px" by simp_all
+      with `(px, Label l') = targetnode a`[THEN sym] 
+      have [simp]:"n = Label l'" "p = px" by simp_all
       with `c \<turnstile> Label l -CEdge (p', es', rets')\<rightarrow>\<^isub>p Label l'` have "l' < #:c"
 	by(fastsimp intro:Proc_CFG_targetlabel_less_num_nodes)
       from `Rep_wf_prog wfp = (prog,procs)` `l' < #:c` 
-	`containsCall procs prog ps px es rets` `(px, ins, outs, c) \<in> set procs`
+	`containsCall procs prog ps px` `(px, ins, outs, c) \<in> set procs`
       obtain as as' where "wfp \<turnstile> (px,Label l') -as\<rightarrow>* (px,Exit)"
 	and "\<forall>a \<in> set as. intra_kind (kind a)"
 	and "wfp \<turnstile> (px,Entry) -as'\<rightarrow>* (px,Label l')"
 	and "\<forall>a \<in> set as'. intra_kind (kind a)"
 	by -(erule Label_Proc_CFG_Entry_Exit_path_Proc)+
       moreover
-      from `Rep_wf_prog wfp = (prog,procs)` `containsCall procs prog ps px es rets`
+      from `Rep_wf_prog wfp = (prog,procs)` `containsCall procs prog ps px`
 	`(px, ins, outs, c) \<in> set procs` obtain asx asx' 
 	where" CFG.valid_path' sourcenode targetnode kind
 	(valid_edge wfp) (get_return_edges wfp) (Main,Entry) asx (px,Entry)"
@@ -2182,11 +2184,12 @@ proof -
     qed
   next
     case (MainCallReturn nx px es rets nx')
-    from `prog \<turnstile> nx -CEdge (px, es, rets)\<rightarrow>\<^isub>p nx'` disj MainCallReturn(3)[THEN sym]
-      MainCallReturn(5)[THEN sym] obtain l where [simp]:"n = Label l" "p = Main"
+    from `prog \<turnstile> nx -CEdge (px, es, rets)\<rightarrow>\<^isub>p nx'` disj
+      `(Main, nx) = sourcenode a`[THEN sym] `(Main, nx') = targetnode a`[THEN sym]
+    obtain l where [simp]:"n = Label l" "p = Main"
       by(fastsimp dest:Proc_CFG_Call_Labels)
-    from `prog \<turnstile> nx -CEdge (px, es, rets)\<rightarrow>\<^isub>p nx'` disj MainCallReturn(3)[THEN sym]
-      MainCallReturn(5)[THEN sym]
+    from `prog \<turnstile> nx -CEdge (px, es, rets)\<rightarrow>\<^isub>p nx'` disj
+      `(Main, nx) = sourcenode a`[THEN sym] `(Main, nx') = targetnode a`[THEN sym]
     have "l < #:prog" by(auto intro:Proc_CFG_sourcelabel_less_num_nodes
       Proc_CFG_targetlabel_less_num_nodes)
     with `Rep_wf_prog wfp = (prog,procs)` 
@@ -2199,17 +2202,19 @@ proof -
       apply(rule_tac x="as" in exI) apply(rule_tac x="as'" in exI) apply simp
       by(fastsimp intro:ProcCFG.intra_path_vp simp:ProcCFG.intra_path_def)
   next
-    case (ProcCallReturn px ins outs c nx p' es' rets' nx' ps es rets)
+    case (ProcCallReturn px ins outs c nx p' es' rets' nx' ps)
     from `(px, ins, outs, c) \<in> set procs` wf have [simp]:"px \<noteq> Main" by auto
-    from `c \<turnstile> nx -CEdge (p', es', rets')\<rightarrow>\<^isub>p nx'` disj ProcCallReturn(5)[THEN sym]
-      ProcCallReturn(7)[THEN sym] obtain l where [simp]:"n = Label l" "p = px"
+    from `c \<turnstile> nx -CEdge (p', es', rets')\<rightarrow>\<^isub>p nx'` disj 
+      `(px, nx) = sourcenode a`[THEN sym] `(px, nx') = targetnode a`[THEN sym]
+    obtain l where [simp]:"n = Label l" "p = px"
       by(fastsimp dest:Proc_CFG_Call_Labels)
-    from `c \<turnstile> nx -CEdge (p', es', rets')\<rightarrow>\<^isub>p nx'` disj ProcCallReturn(5)[THEN sym]
-      ProcCallReturn(7)[THEN sym] have "l < #:c"
+    from `c \<turnstile> nx -CEdge (p', es', rets')\<rightarrow>\<^isub>p nx'` disj 
+    `(px, nx) = sourcenode a`[THEN sym] `(px, nx') = targetnode a`[THEN sym]
+    have "l < #:c"
       by(auto intro:Proc_CFG_sourcelabel_less_num_nodes
 	Proc_CFG_targetlabel_less_num_nodes)
     with `Rep_wf_prog wfp = (prog,procs)` `(px, ins, outs, c) \<in> set procs` 
-      `containsCall procs prog ps px es rets`
+      `containsCall procs prog ps px`
     obtain as as' where "wfp \<turnstile> (px,Entry) -as\<rightarrow>* (px,Label l)"
       and "\<forall>a \<in> set as. intra_kind (kind a)"
       and "wfp \<turnstile> (px,Label l) -as'\<rightarrow>* (px,Exit)"
@@ -2217,7 +2222,7 @@ proof -
       by -(erule Label_Proc_CFG_Entry_Exit_path_Proc)+
     moreover
     from `Rep_wf_prog wfp = (prog,procs)` 
-      `containsCall procs prog ps px es rets` `(px, ins, outs, c) \<in> set procs`
+      `containsCall procs prog ps px` `(px, ins, outs, c) \<in> set procs`
     obtain asx asx' where "CFG.valid_path' sourcenode targetnode kind
       (valid_edge wfp) (get_return_edges wfp) (Main,Entry) asx (px,Entry)"
       and "CFG.valid_path' sourcenode targetnode kind
@@ -2345,4 +2350,3 @@ qed
 
 
 end
-
